Proved all rules CSL IDF, some sorrys to remove

simple-frontend/CSL_IDF.thy
@@ -4,167 +4,161 @@ begin
 
 subsection \<open>Safety\<close>
 
-definition binary_mask where
-  "binary_mask \<omega> \<longleftrightarrow> (\<forall>l. get_m \<omega> l = 0 \<or> get_m \<omega> l = 1)"
-
-definition concretize :: "int equi_state \<Rightarrow> state" where                                              
-  "concretize \<omega> = (get_store \<omega>, get_h \<omega>)"
-
-definition read_dom where 
-  "read_dom \<omega> = { l. get_m \<omega> (l, field_val) > 0 }"
-
-definition write_dom where 
-  "write_dom \<omega> = { l. get_m \<omega> (l, field_val) = 1 }"
-
-definition no_aborts where
-  "no_aborts C \<omega>0 \<longleftrightarrow> (\<forall>\<omega>0' \<omega>f. sep_algebra_class.stable \<omega>f \<and> Some \<omega>0' = \<omega>0 \<oplus> \<omega>f \<and> binary_mask \<omega>0' \<longrightarrow> \<not> aborts C (concretize \<omega>0'))"
-
-lemma no_abortsI[intro]:
-  assumes "\<And>\<omega>0' \<omega>f. sep_algebra_class.stable \<omega>f \<Longrightarrow> Some \<omega>0' = \<omega>0 \<oplus> \<omega>f \<and> binary_mask \<omega>0' \<Longrightarrow> \<not> aborts C (concretize \<omega>0')"
-  shows "no_aborts C \<omega>0"
-  using assms no_aborts_def by blast
-
 (*
-inductive
-  aborts :: "cmd \<Rightarrow> state \<Rightarrow> bool"
-where
-  aborts_Seq[intro]:   "aborts C1 \<sigma> \<Longrightarrow> aborts (Cseq C1 C2) \<sigma>" 
-| aborts_Par1[intro]:  "aborts C1 \<sigma> \<Longrightarrow> aborts (Cpar C1 C2) \<sigma>" 
-| aborts_Par2[intro]:  "aborts C2 \<sigma> \<Longrightarrow> aborts (Cpar C1 C2) \<sigma>"
-
-| aborts_Race1[intro]:  "\<not> disjoint (accesses C1 (fst \<sigma>)) (writes C2 (fst \<sigma>)) \<Longrightarrow> aborts (Cpar C1 C2) \<sigma>"
-| aborts_Race2[intro]:  "\<not> disjoint (writes C1 (fst \<sigma>)) (accesses C2 (fst \<sigma>)) \<Longrightarrow> aborts (Cpar C1 C2) \<sigma>"
-
-| aborts_Read[intro]:  "\<lbrakk> fst \<sigma> r = Some (VRef (Address l)); (l, field_val) \<notin> dom (snd \<sigma>) \<rbrakk> \<Longrightarrow> aborts (Cread x r) \<sigma>"
-| aborts_Write[intro]: "\<lbrakk> fst \<sigma> r = Some (VRef (Address l)); (l, field_val) \<notin> dom (snd \<sigma>) \<rbrakk> \<Longrightarrow> aborts (Cwrite r E) \<sigma>"
-| aborts_Free[intro]:  "\<lbrakk> fst \<sigma> r = Some (VRef (Address l)); (l, field_val) \<notin> dom (snd \<sigma>) \<rbrakk> \<Longrightarrow> aborts (Cdispose r) \<sigma>"
-
-| aborts_ReadNull[intro]: "fst \<sigma> r = Some (VRef Null) \<Longrightarrow> aborts (Cread x r) \<sigma>"
-| aborts_WriteNull[intro]: "fst \<sigma> r = Some (VRef Null) \<Longrightarrow> aborts (Cwrite r e) \<sigma>"
-| aborts_FreeNull[intro]: "fst \<sigma> r = Some (VRef Null) \<Longrightarrow> aborts (Cdispose r) \<sigma>"
+('a ag_trace \<times> 'a virtual_state)
+*)
+(*
+type_synonym pheap = "int ag_trace \<times> int virtual_state"
 *)
 
-(* Probably should be stable somewhere *)
+definition binary_mask where
+  "binary_mask \<omega> \<longleftrightarrow> (\<forall>l. get_vm \<omega> l = 0 \<or> get_vm \<omega> l = 1)"
+
+lemma binary_maskI:
+  assumes "\<And>l. get_vm \<omega> l = 0 \<or> get_vm \<omega> l = 1"
+  shows "binary_mask \<omega>"
+  using assms binary_mask_def by blast
+
+abbreviation concretize where                                              
+  "concretize s \<omega> \<equiv> (s, get_vh \<omega>)"
+
+definition read_dom where 
+  "read_dom \<omega> = { l. get_vm \<omega> (l, field_val) > 0 }"
+
+definition write_dom where 
+  "write_dom \<omega> = { l. get_vm \<omega> (l, field_val) = 1 }"
+
+definition no_aborts where
+  "no_aborts C s0 \<omega>0 \<longleftrightarrow> (\<forall>\<omega>0' \<omega>f. sep_algebra_class.stable \<omega>f \<and> Some \<omega>0' = \<omega>0 \<oplus> \<omega>f \<and> binary_mask \<omega>0' \<longrightarrow> \<not> aborts C (s0, get_vh \<omega>0'))"
+
+lemma no_abortsI[intro]:
+  assumes "\<And>\<omega>0' \<omega>f. sep_algebra_class.stable \<omega>f \<Longrightarrow> Some \<omega>0' = \<omega>0 \<oplus> \<omega>f \<and> binary_mask \<omega>0' \<Longrightarrow> \<not> aborts C (s0, get_vh \<omega>0')"
+  shows "no_aborts C s0 \<omega>0"
+  using assms no_aborts_def by blast
+
+
+(*
+type_synonym 'v ag_store = "(var \<rightharpoonup> 'v) agreement"
+type_synonym ('v, 'a) abs_state = "'v ag_store \<times> 'a"
+('a val, ('a ag_trace \<times> 'a virtual_state)) abs_state"
+*)
+
  primrec
-  safe :: "nat \<Rightarrow> cmd \<Rightarrow> int equi_state \<Rightarrow> int equi_state set \<Rightarrow> bool"
+  safe :: "nat \<Rightarrow> cmd \<Rightarrow> stack \<Rightarrow> int ag_trace \<Rightarrow> int virtual_state \<Rightarrow> int equi_state set \<Rightarrow> bool"
 where
-  "safe 0 C \<omega> Q \<longleftrightarrow> True"
-| "safe (Suc n) C \<omega>0 Q \<longleftrightarrow>
-  (C = Cskip \<longrightarrow> \<omega>0 \<in> Q)
-  \<and> accesses C (get_store \<omega>0) \<subseteq> read_dom \<omega>0
-  \<and> writes C (get_store \<omega>0) \<subseteq> write_dom \<omega>0
-  \<and> no_aborts C \<omega>0
+  "safe 0 C s \<tau> \<omega> Q \<longleftrightarrow> True"
+| "safe (Suc n) C s0 \<tau> \<omega>0 Q \<longleftrightarrow>
+  (C = Cskip \<longrightarrow> (Ag s0, \<tau>, \<omega>0) \<in> Q)
+  \<and> accesses C s0 \<subseteq> read_dom \<omega>0
+  \<and> writes C s0 \<subseteq> write_dom \<omega>0
+  \<and> no_aborts C s0 \<omega>0
   \<and> (\<forall>\<omega>0' \<omega>f C' \<sigma>'. sep_algebra_class.stable \<omega>f \<and> Some \<omega>0' = \<omega>0 \<oplus> \<omega>f \<and> binary_mask \<omega>0' \<and>
-  (\<langle>C, concretize \<omega>0'\<rangle> \<rightarrow> \<langle>C', \<sigma>'\<rangle>)
-\<longrightarrow> (\<exists>\<omega>1 \<omega>1'. Some \<omega>1' = \<omega>1 \<oplus> \<omega>f \<and> sep_algebra_class.stable \<omega>1 \<and> binary_mask \<omega>1' \<and> \<sigma>' = concretize \<omega>1' \<and> safe n C' \<omega>1 Q))"
+  (\<langle>C, concretize s0 \<omega>0'\<rangle> \<rightarrow> \<langle>C', \<sigma>'\<rangle>)
+\<longrightarrow> (\<exists>\<omega>1 \<omega>1'. Some \<omega>1' = \<omega>1 \<oplus> \<omega>f \<and> sep_algebra_class.stable \<omega>1 \<and> binary_mask \<omega>1' \<and> snd \<sigma>' = get_vh \<omega>1' \<and> safe n C' (fst \<sigma>') \<tau> \<omega>1 Q))"
 
 lemma safeI:
-  assumes "C = Cskip \<Longrightarrow> \<omega>0 \<in> Q"
-      and "accesses C (get_store \<omega>0) \<subseteq> read_dom \<omega>0"
-      and "writes C (get_store \<omega>0) \<subseteq> write_dom \<omega>0"
-      and "no_aborts C \<omega>0"
-      and "\<And>\<omega>0' \<omega>f C' \<sigma>'. sep_algebra_class.stable \<omega>f \<Longrightarrow> Some \<omega>0' = \<omega>0 \<oplus> \<omega>f \<and> binary_mask \<omega>0' \<and>
-  (\<langle>C, concretize \<omega>0'\<rangle> \<rightarrow> \<langle>C', \<sigma>'\<rangle>)
-\<Longrightarrow> (\<exists>\<omega>1 \<omega>1'. Some \<omega>1' = \<omega>1 \<oplus> \<omega>f \<and> sep_algebra_class.stable \<omega>1 \<and> binary_mask \<omega>1' \<and> \<sigma>' = concretize \<omega>1' \<and> safe n C' \<omega>1 Q)"
-    shows "safe (Suc n) C \<omega>0 Q"
+  assumes "C = Cskip \<Longrightarrow> (Ag s0, \<tau>, \<omega>0) \<in> Q"
+      and "accesses C s0 \<subseteq> read_dom \<omega>0"
+      and "writes C s0 \<subseteq> write_dom \<omega>0"
+      and "no_aborts C s0 \<omega>0"
+      and "\<And>\<omega>0' \<omega>f C' \<sigma>'. sep_algebra_class.stable \<omega>f \<Longrightarrow> Some \<omega>0' = \<omega>0 \<oplus> \<omega>f \<Longrightarrow> binary_mask \<omega>0' \<Longrightarrow>
+  (\<langle>C, concretize s0 \<omega>0'\<rangle> \<rightarrow> \<langle>C', \<sigma>'\<rangle>)
+\<Longrightarrow> (\<exists>\<omega>1 \<omega>1'. Some \<omega>1' = \<omega>1 \<oplus> \<omega>f \<and> sep_algebra_class.stable \<omega>1 \<and> binary_mask \<omega>1' \<and> snd \<sigma>' = get_vh \<omega>1' \<and> safe n C' (fst \<sigma>') \<tau> \<omega>1 Q)"
+    shows "safe (Suc n) C s0 \<tau> \<omega>0 Q"
   using assms safe.simps(1) by auto
 
 
 lemma safeI_alt:
-  assumes "C = Cskip \<Longrightarrow> \<omega>0 \<in> Q"
-      and "accesses C (get_store \<omega>0) \<subseteq> read_dom \<omega>0"
-      and "writes C (get_store \<omega>0) \<subseteq> write_dom \<omega>0"
-      and "\<And>\<omega>0' \<omega>f. sep_algebra_class.stable \<omega>f \<Longrightarrow> Some \<omega>0' = \<omega>0 \<oplus> \<omega>f \<and> binary_mask \<omega>0' \<Longrightarrow> aborts C (concretize \<omega>0') \<Longrightarrow> False"
-      and "\<And>\<omega>0' \<omega>f C' \<sigma>'. sep_algebra_class.stable \<omega>f \<Longrightarrow> Some \<omega>0' = \<omega>0 \<oplus> \<omega>f \<and> binary_mask \<omega>0' \<Longrightarrow>
-  (\<langle>C, concretize \<omega>0'\<rangle> \<rightarrow> \<langle>C', \<sigma>'\<rangle>)
-\<Longrightarrow> (\<exists>\<omega>1 \<omega>1'. Some \<omega>1' = \<omega>1 \<oplus> \<omega>f \<and> sep_algebra_class.stable \<omega>1 \<and> binary_mask \<omega>1' \<and> \<sigma>' = concretize \<omega>1' \<and> safe n C' \<omega>1 Q)"
-    shows "safe (Suc n) C \<omega>0 Q"
+  assumes "C = Cskip \<Longrightarrow> (Ag s0, \<tau>, \<omega>0) \<in> Q"
+      and "accesses C s0 \<subseteq> read_dom \<omega>0"
+      and "writes C s0 \<subseteq> write_dom \<omega>0"
+      and "\<And>\<omega>0' \<omega>f. sep_algebra_class.stable \<omega>f \<Longrightarrow> Some \<omega>0' = \<omega>0 \<oplus> \<omega>f \<Longrightarrow> binary_mask \<omega>0' \<Longrightarrow> aborts C (concretize s0 \<omega>0') \<Longrightarrow> False"
+      and "\<And>\<omega>0' \<omega>f C' \<sigma>'. sep_algebra_class.stable \<omega>f \<Longrightarrow> Some \<omega>0' = \<omega>0 \<oplus> \<omega>f \<Longrightarrow> binary_mask \<omega>0' \<Longrightarrow>
+  (\<langle>C, concretize s0 \<omega>0'\<rangle> \<rightarrow> \<langle>C', \<sigma>'\<rangle>)
+\<Longrightarrow> (\<exists>\<omega>1 \<omega>1'. Some \<omega>1' = \<omega>1 \<oplus> \<omega>f \<and> sep_algebra_class.stable \<omega>1 \<and> binary_mask \<omega>1' \<and> snd \<sigma>' = get_vh \<omega>1' \<and> safe n C' (fst \<sigma>') \<tau> \<omega>1 Q)"
+    shows "safe (Suc n) C s0 \<tau> \<omega>0 Q"
   using assms safe.simps(1) 
   by fastforce
 
 lemma safeE:
-  assumes "safe (Suc n) C \<omega>0 Q"
-  shows "C = Cskip \<Longrightarrow> \<omega>0 \<in> Q"
-      and "accesses C (get_store \<omega>0) \<subseteq> read_dom \<omega>0"
-      and "writes C (get_store \<omega>0) \<subseteq> write_dom \<omega>0"
-      and "no_aborts C \<omega>0"
-      and "sep_algebra_class.stable \<omega>f \<and> Some \<omega>0' = \<omega>0 \<oplus> \<omega>f \<and> binary_mask \<omega>0' \<and> (\<langle>C, concretize \<omega>0'\<rangle> \<rightarrow> \<langle>C', \<sigma>'\<rangle>)
-\<Longrightarrow> (\<exists>\<omega>1 \<omega>1'. Some \<omega>1' = \<omega>1 \<oplus> \<omega>f \<and> sep_algebra_class.stable \<omega>1 \<and> binary_mask \<omega>1' \<and> \<sigma>' = concretize \<omega>1' \<and> safe n C' \<omega>1 Q)"
+  assumes "safe (Suc n) C s0 \<tau> \<omega>0 Q"
+  shows "C = Cskip \<Longrightarrow> (Ag s0, \<tau>, \<omega>0) \<in> Q"
+      and "accesses C s0 \<subseteq> read_dom \<omega>0"
+      and "writes C s0 \<subseteq> write_dom \<omega>0"
+      and "no_aborts C s0 \<omega>0"
+      and "sep_algebra_class.stable \<omega>f \<and> Some \<omega>0' = \<omega>0 \<oplus> \<omega>f \<and> binary_mask \<omega>0' \<and> (\<langle>C, concretize s0 \<omega>0'\<rangle> \<rightarrow> \<langle>C', \<sigma>'\<rangle>)
+\<Longrightarrow> (\<exists>\<omega>1 \<omega>1'. Some \<omega>1' = \<omega>1 \<oplus> \<omega>f \<and> sep_algebra_class.stable \<omega>1 \<and> binary_mask \<omega>1' \<and> snd \<sigma>' = get_vh \<omega>1' \<and> safe n C' (fst \<sigma>') \<tau> \<omega>1 Q)"
   using assms safe.simps(1) apply simp_all
   by (metis prod.collapse)
 
 
-definition CSL where
-  "CSL P C Q \<longleftrightarrow> (\<forall>n \<omega>. \<omega> \<in> P \<and> sep_algebra_class.stable \<omega> \<longrightarrow> safe n C \<omega> Q)"
+definition CSL :: "int equi_state set \<Rightarrow> cmd \<Rightarrow> int equi_state set \<Rightarrow> bool" where
+  "CSL P C Q \<longleftrightarrow> (\<forall>n s \<tau> \<omega>. (Ag s, \<tau>, \<omega>) \<in> P \<and> sep_algebra_class.stable \<omega> \<longrightarrow> safe n C s \<tau> \<omega> Q)"
 
 lemma CSL_I:
-  assumes "\<And>n \<omega>. \<omega> \<in> P \<Longrightarrow> sep_algebra_class.stable \<omega> \<Longrightarrow> safe n C \<omega> Q"
+  assumes "\<And>n s \<tau> \<omega>. (Ag s, \<tau>, \<omega>) \<in> P \<Longrightarrow> sep_algebra_class.stable \<omega> \<Longrightarrow> safe (Suc n) C s \<tau> \<omega> Q"
   shows "CSL P C Q"
-  by (simp add: CSL_def assms)
+  by (metis CSL_def assms not0_implies_Suc safe.simps(1))
 
 lemma CSL_E:
   assumes "CSL P C Q"
-      and "\<omega> \<in> P"
+      and "(Ag s, \<tau>, \<omega>) \<in> P"
       and "sep_algebra_class.stable \<omega>"
-    shows "safe n C \<omega> Q"
-  using CSL_def assms by blast
+    shows "safe n C s \<tau> \<omega> Q"
+  using CSL_def assms by fast
 
 
 lemma safety_mono:
-  assumes "safe n C \<omega> Q"
+  assumes "safe n C s \<tau> \<omega> Q"
       and "m \<le> n"
-    shows "safe m C \<omega> Q"
+    shows "safe m C s \<tau> \<omega> Q"
   using assms
-proof (induct m arbitrary: C n \<omega>)
+proof (induct m arbitrary: C n s \<omega>)
   case (Suc m)
   then obtain k where "n = Suc k"
     using Suc_le_D by presburger
-  then show ?case using safeI[of C \<omega> Q] safeE
+  then show ?case using safeI[of C s \<tau> \<omega> Q] safeE
     by (smt (verit, ccfv_threshold) Suc.hyps Suc.prems(1) Suc.prems(2) Suc_le_mono)
 qed (simp)
 
 (* TODO: Need to define the fvA Q... *)
 
 lemma no_aborts_agrees:
-  assumes "no_aborts C \<omega>"
-      and "agrees (fvC C) (get_store \<omega>) (get_store \<omega>')"
-      and "get_state \<omega> = get_state \<omega>'"
-    shows "no_aborts C \<omega>'"
+  assumes "no_aborts C s \<omega>"
+      and "agrees (fvC C) s s'"
+    shows "no_aborts C s' \<omega>"
   sorry
 
 definition fvA where
   "fvA Q = undefined Q"
 
 lemma fvA_agrees:
-  assumes "agrees (fvA Q) (get_store \<omega>) (get_store \<omega>')"
-      and "get_state \<omega> = get_state \<omega>'"
-    shows "\<omega> \<in> Q \<longleftrightarrow> \<omega>' \<in> Q"
+  assumes "agrees (fvA Q) s s'"
+    shows "(Ag s, \<tau>, \<omega>) \<in> Q \<longleftrightarrow> (Ag s', \<tau>, \<omega>) \<in> Q"
   sorry
 
 lemma safe_agrees:
-  assumes "safe n C \<omega> Q"
-      and "agrees (fvC C \<union> fvA Q) (get_store \<omega>) (get_store \<omega>')"
-      and "get_state \<omega> = get_state \<omega>'"
-    shows "safe n C \<omega>' Q"
+  assumes "safe n C s \<tau> \<omega> Q"
+      and "agrees (fvC C \<union> fvA Q) s s'"
+    shows "safe n C s' \<tau> \<omega> Q"
   using assms
-proof (induct n arbitrary: C \<omega> \<omega>')
+proof (induct n arbitrary: C s s' \<omega>)
   case (Suc n)
   show ?case
   proof (rule safeI)
-    have "C = Cskip \<Longrightarrow> \<omega> \<in> Q"
-      using Suc.prems(1) safe.simps(2) by blast
-    then show "C = Cskip \<Longrightarrow> \<omega>' \<in> Q"
-      using Suc.prems(2) Suc.prems(3) agrees_simps(4) fvA_agrees by blast
-    show "accesses C (get_store \<omega>') \<subseteq> read_dom \<omega>'"
-      by (metis Suc.prems(1) Suc.prems(2) Suc.prems(3) accesses_agrees agrees_simps(4) read_dom_def safeE(2))
-    show "writes C (get_store \<omega>') \<subseteq> write_dom \<omega>'"
-      by (metis Suc.prems(1) Suc.prems(2) Suc.prems(3) agrees_simps(4) safeE(3) write_dom_def writes_agrees)
-    show "no_aborts C \<omega>'"
-      using Suc.prems(1) Suc.prems(2) Suc.prems(3) agrees_simps(4) no_aborts_agrees safe.simps(2) by blast
+    show "C = Cskip \<Longrightarrow> (Ag s', \<tau>, \<omega>) \<in> Q"
+      using safeE(1)[OF Suc.prems(1)]
+      by (meson Suc.prems(2) agrees_simps(4) fvA_agrees)
+    show "accesses C s' \<subseteq> read_dom \<omega>"
+      using Suc.prems(1) Suc.prems(2) accesses_agrees by force
+    show "writes C s' \<subseteq> write_dom \<omega>"
+      using Suc.prems(1) Suc.prems(2) agrees_simps(4) safeE(3) writes_agrees by blast
+    show "no_aborts C s' \<omega>"
+      by (meson Suc.prems(1) Suc.prems(2) agrees_simps(4) no_aborts_agrees safeE(4))
     fix \<omega>0' \<omega>f C' \<sigma>'
-    assume asm0: "sep_algebra_class.stable \<omega>f" "Some \<omega>0' = \<omega>' \<oplus> \<omega>f \<and> binary_mask \<omega>0' \<and> \<langle>C, concretize \<omega>0'\<rangle> \<rightarrow> \<langle>C', \<sigma>'\<rangle>"
+    assume asm0: "sep_algebra_class.stable \<omega>f" "Some \<omega>0' = \<omega> \<oplus> \<omega>f" "binary_mask \<omega>0'" "\<langle>C, concretize s' \<omega>0'\<rangle> \<rightarrow> \<langle>C', \<sigma>'\<rangle>"
 
-    show "\<exists>\<omega>1 \<omega>1'. Some \<omega>1' = \<omega>1 \<oplus> \<omega>f \<and> sep_algebra_class.stable \<omega>1 \<and> binary_mask \<omega>1' \<and> \<sigma>' = concretize \<omega>1' \<and> safe n C' \<omega>1 Q"
+    then show "\<exists>\<omega>1 \<omega>1'. Some \<omega>1' = \<omega>1 \<oplus> \<omega>f \<and> sep_algebra_class.stable \<omega>1 \<and> binary_mask \<omega>1' \<and> snd \<sigma>' = get_vh \<omega>1' \<and> safe n C' (fst \<sigma>') \<tau> \<omega>1 Q"
       sorry
   qed
 qed (simp)
@@ -174,26 +168,28 @@ qed (simp)
 subsection \<open>Skip\<close>
 
 lemma safe_skip[intro!]:
-  assumes "\<omega> \<in> Q"
-  shows "safe n Cskip \<omega> Q"
+  assumes "(Ag s, \<tau>, \<omega>) \<in> Q"
+  shows "safe n Cskip s \<tau> \<omega> Q"
 proof (induct n)
   case (Suc n)
   show ?case
   proof (rule safeI)
-    show "no_aborts Cskip \<omega>"
+    show "no_aborts Cskip s \<omega>"
       by (simp add: no_abortsI)
-    show "Cskip = Cskip \<Longrightarrow> \<omega> \<in> Q"
+    show "Cskip = Cskip \<Longrightarrow> (Ag s, \<tau>, \<omega>) \<in> Q"
       by (simp add: assms)
     fix \<omega>0' \<omega>f C' \<sigma>'
-    assume "Some \<omega>0' = \<omega> \<oplus> \<omega>f \<and> binary_mask \<omega>0' \<and> \<langle>Cskip, concretize \<omega>0'\<rangle> \<rightarrow> \<langle>C', \<sigma>'\<rangle>"
-    show "\<exists>\<omega>1 \<omega>1'. Some \<omega>1' = \<omega>1 \<oplus> \<omega>f \<and> sep_algebra_class.stable \<omega>1 \<and> binary_mask \<omega>1' \<and> \<sigma>' = concretize \<omega>1' \<and> safe n C' \<omega>1 Q"
-      using \<open>Some \<omega>0' = \<omega> \<oplus> \<omega>f \<and> binary_mask \<omega>0' \<and> \<langle>Cskip, concretize \<omega>0'\<rangle> \<rightarrow> \<langle>C', \<sigma>'\<rangle>\<close> by auto
+    assume "\<langle>Cskip, concretize s \<omega>0'\<rangle> \<rightarrow> \<langle>C', \<sigma>'\<rangle>"
+    then show "\<exists>\<omega>1 \<omega>1'. Some \<omega>1' = \<omega>1 \<oplus> \<omega>f \<and> sep_algebra_class.stable \<omega>1 \<and> binary_mask \<omega>1' \<and> snd \<sigma>' = get_vh \<omega>1' \<and> safe n C' (fst \<sigma>') \<tau> \<omega>1 Q"
+      by force
   qed (simp_all)
 qed (simp)
 
 proposition rule_skip:
   "CSL P Cskip P"
-  by (simp add: CSL_def safe_skip)
+  using CSL_def by blast
+
+
 
 
 subsection \<open>Frame rule\<close>
@@ -209,95 +205,11 @@ lemma write_dom_mono:
   sorry
 
 lemma no_aborts_mono:
-  assumes "no_aborts C \<omega>"
+  assumes "no_aborts C s \<omega>"
       and "\<omega>' \<succeq> \<omega>"
-    shows "no_aborts C \<omega>'"
+    shows "no_aborts C s \<omega>'"
   sorry
 
-lemma frame_safe:
-  assumes "safe n C \<omega> Q"
-      and "fvA R \<inter> wrC C = {}"
-      and "Some \<omega>' = \<omega> \<oplus> \<omega>f"
-      and "\<omega>f \<in> R"
-      and "sep_algebra_class.stable \<omega>f"
-    shows "safe n C \<omega>' (Q \<otimes> R)"
-  using assms
-proof (induct n arbitrary: C \<omega> \<omega>' \<omega>f)
-  case (Suc n)
-  show ?case
-  proof (rule safeI)
-    show "C = Cskip \<Longrightarrow> \<omega>' \<in> Q \<otimes> R"
-      by (metis Suc.prems(1) Suc.prems(3) Suc.prems(4) safeE(1) x_elem_set_product)
-    show "accesses C (get_store \<omega>') \<subseteq> read_dom \<omega>'"
-      by (metis (no_types, lifting) Suc.prems(1) Suc.prems(3) Suc.prems(4) dual_order.trans full_add_charact(1) in_set_sum is_in_set_sum read_dom_mono safeE(2) singletonD)
-    show "writes C (get_store \<omega>') \<subseteq> write_dom \<omega>'"
-      by (metis (no_types, lifting) Suc.prems(1) Suc.prems(3) full_add_charact(1) greater_def inf.absorb_iff2 inf.coboundedI1 safeE(3) write_dom_mono)
-    show "no_aborts C \<omega>'"
-      by (meson Suc.prems(1) Suc.prems(3) greater_def no_aborts_mono safeE(4))
-    fix \<omega>0' \<omega>f' C' \<sigma>'
-    assume asm0: "sep_algebra_class.stable \<omega>f'" "Some \<omega>0' = \<omega>' \<oplus> \<omega>f' \<and> binary_mask \<omega>0' \<and> \<langle>C, concretize \<omega>0'\<rangle> \<rightarrow> \<langle>C', \<sigma>'\<rangle>"
-    then obtain \<omega>f'' where "Some \<omega>f'' = \<omega>f \<oplus> \<omega>f'"
-      by (metis (no_types, opaque_lifting) Suc.prems(3) asso2 option.collapse)
-    then have "Some \<omega>0' = \<omega> \<oplus> \<omega>f''"
-      using asm0 Suc.prems(3) asso1 by force
-    then obtain \<omega>1'' \<omega>1' where "Some \<omega>1' = \<omega>1'' \<oplus> \<omega>f'' \<and> binary_mask \<omega>1' \<and> \<sigma>' = concretize \<omega>1'" "safe n C' \<omega>1'' Q" "sep_algebra_class.stable \<omega>1''"
-      using safeE(5)[OF Suc(2), of \<omega>0' \<omega>f'' C' \<sigma>'] asm0 
-      by (meson Suc.prems(1) Suc.prems(5) \<open>Some \<omega>f'' = \<omega>f \<oplus> \<omega>f'\<close> safeE(5) stable_sum)
-    then obtain \<omega>1 where "Some \<omega>1 = \<omega>1'' \<oplus> \<omega>f"
-      by (metis (no_types, opaque_lifting) \<open>Some \<omega>f'' = \<omega>f \<oplus> \<omega>f'\<close> asso3 option.collapse)
-    moreover have "safe n C' \<omega>1 (Q \<otimes> R)"
-      using \<open>safe n C' \<omega>1'' Q\<close>
-    proof (rule Suc(1)[of C' \<omega>1'' \<omega>1 \<omega>f])
-      show "fvA R \<inter> wrC C' = {}"
-        by (meson Suc.prems(2) asm0 disjoint_iff red_properties subset_iff)
-      show "Some \<omega>1 = \<omega>1'' \<oplus> \<omega>f"
-        using calculation by auto
-    qed (simp_all add: Suc.prems)
-    ultimately show "\<exists>\<omega>1 \<omega>1'. Some \<omega>1' = \<omega>1 \<oplus> \<omega>f' \<and> sep_algebra_class.stable \<omega>1 \<and> binary_mask \<omega>1' \<and> \<sigma>' = concretize \<omega>1' \<and> safe n C' \<omega>1 (Q \<otimes> R)"
-      by (metis (no_types, lifting) Suc.prems(5) \<open>Some \<omega>1' = \<omega>1'' \<oplus> \<omega>f'' \<and> binary_mask \<omega>1' \<and> \<sigma>' = concretize \<omega>1'\<close> \<open>Some \<omega>f'' = \<omega>f \<oplus> \<omega>f'\<close> \<open>sep_algebra_class.stable \<omega>1''\<close> asso1 stable_sum)
-  qed
-qed (simp)
-
-(*
-lemma self_framing_wf_split:
-  assumes "\<omega> \<in> A \<otimes> B"
-      and "TypedEqui.wf_assertion \<Delta> A"
-      and "self_framing B"
-    shows "\<exists>a b. a \<in> A \<and> b \<in> B \<and> Some \<omega> = a \<oplus> b \<and> sep_algebra_class.stable b"
-proof -
-  obtain a b where "Some \<omega> = a \<oplus> b" "a \<in> A" "b \<in> B"
-    by (meson assms(1) x_elem_set_product)
-  then obtain a' where "Some a' = a \<oplus> |\<omega>|"
-    by (metis commutative minus_equiv_def_any_elem)
-  then have "Some \<omega> = a' \<oplus> stabilize b"
-    by (smt (verit, best) \<open>Some \<omega> = a \<oplus> b\<close> asso1 commutative core_is_pure core_is_smaller core_sum decompose_stabilize_pure)
-  then show ?thesis
-    by (metis (no_types, opaque_lifting) TypedEqui.wf_assertion_def \<open>Some a' = a \<oplus> |\<omega>|\<close> \<open>a \<in> A\<close> \<open>b \<in> B\<close> assms(2) assms(3) core_is_pure in_Stabilize pure_def pure_larger_def self_framing_eq stabilize_is_stable)
-qed
-*)
-
-proposition frame_rule:
-  assumes "CSL P C Q"
-      and "disjoint (fvA R) (wrC C)"
-      and "self_framing P"
-      and "self_framing R"
-    shows "CSL (P \<otimes> R) C (Q \<otimes> R)"
-proof (rule CSL_I)
-  fix n \<omega> assume "\<omega> \<in> P \<otimes> R" "sep_algebra_class.stable \<omega>"
-  then obtain \<omega>p \<omega>r where r: "Some \<omega> = \<omega>p \<oplus> \<omega>r" "\<omega>p \<in> P" "\<omega>r \<in> R"
-    by (meson x_elem_set_product)
-  then have "Some \<omega> = stabilize \<omega>p \<oplus> stabilize \<omega>r"
-    using \<open>sep_algebra_class.stable \<omega>\<close> stabilize_sum_of_stable by blast
-  then show "safe n C \<omega> (Q \<otimes> R)"
-    using frame_safe[of n C "stabilize \<omega>p" Q R \<omega> "stabilize \<omega>r"]
-    by (meson CSL_E assms(1) assms(2) assms(3) assms(4) disjoint_def r(2) r(3) self_framing_def stabilize_is_stable)
-qed
-
-
-subsection \<open>Rule FieldAssign\<close>
-
-abbreviation update_heap_val where
-  "update_heap_val \<omega> l v \<equiv> set_state \<omega> (set_value (get_state \<omega>) l v)"
 
 lemma compatibleI:
   assumes "get_store a = get_store b"
@@ -327,146 +239,129 @@ proof -
 qed
 
 
-lemma write_helper:
-  assumes "Some \<omega>' = \<omega> \<oplus> \<omega>f"
-      and "sep_algebra_class.stable \<omega>f"
-      and "get_m \<omega> l = 1"
-    shows "Some (update_heap_val \<omega>' l v) = update_heap_val \<omega> l v \<oplus> \<omega>f"
-proof -
-  have "get_m \<omega>' l = get_m \<omega> l + get_m \<omega>f l"
-    by (meson assms(1) get_m_additive)
-  moreover have "get_m \<omega>' l \<le> 1" sorry
-  ultimately have "get_m \<omega>f l = 0"
-    by (metis PosReal.padd_cancellative add.commute add.right_neutral assms(3) nle_le pos_perm_class.sum_larger)
-  moreover have "get_h \<omega>f l = None" (* TODO: Extract as lemma *)
-  proof -
-    have "sep_algebra_class.stable (get_state \<omega>f)"
-      using stable_prod_def
-      by (metis assms(2) get_state_def)
-    then show ?thesis using stable_virtual_state_def[of "get_state \<omega>f"]
-      using calculation pperm_pgt_pnone by blast
-  qed
-  show "Some (update_heap_val \<omega>' l v) = update_heap_val \<omega> l v \<oplus> \<omega>f"
-  proof (rule sum_equi_statesI)
-    show "get_store (update_heap_val \<omega>' l v) = get_store (update_heap_val \<omega> l v)"
-      by (simp add: assms(1) full_add_charact(1))
-    show "get_store (update_heap_val \<omega>' l v) = get_store \<omega>f"
-      by (metis assms(1) commutative full_add_charact(1) get_store_set_state)
-    show "get_trace (update_heap_val \<omega>' l v) = get_trace (update_heap_val \<omega> l v)"
-      by (metis assms(1) get_trace_set_state greater_def greater_state_has_greater_parts(2))
-    show "get_trace (update_heap_val \<omega>' l v) = get_trace \<omega>f"
-      by (metis assms(1) get_trace_set_state greater_equiv greater_state_has_greater_parts(2))
-    show "Some (get_state (update_heap_val \<omega>' l v)) = get_state (update_heap_val \<omega> l v) \<oplus> get_state \<omega>f"
-    proof (rule compatible_virtual_state_implies_pre_virtual_state_rev)
-      show "Some (Rep_virtual_state (get_state (update_heap_val \<omega>' l v))) =
-    Rep_virtual_state (get_state (update_heap_val \<omega> l v)) \<oplus> Rep_virtual_state (get_state \<omega>f)"
-      proof (rule plus_prodI)
-        show "Some (fst (Rep_virtual_state (get_state (update_heap_val \<omega>' l v)))) =
-    fst (Rep_virtual_state (get_state (update_heap_val \<omega> l v))) \<oplus> fst (Rep_virtual_state (get_state \<omega>f))"
-          by (metis assms(1) get_state_set_state get_vm_additive get_vm_def set_value_charact(1) state_add_iff)
-        show "Some (snd (Rep_virtual_state (get_state (update_heap_val \<omega>' l v)))) =
-    snd (Rep_virtual_state (get_state (update_heap_val \<omega> l v))) \<oplus> snd (Rep_virtual_state (get_state \<omega>f))"
-        proof (rule plus_funI)
-          fix la show "Some (snd (Rep_virtual_state (get_state (update_heap_val \<omega>' l v))) la) =
-          snd (Rep_virtual_state (get_state (update_heap_val \<omega> l v))) la \<oplus> snd (Rep_virtual_state (get_state \<omega>f)) la"
-          proof (cases "l = la")
-            case True
-            then have "snd (Rep_virtual_state (get_state (update_heap_val \<omega>' l v))) la = Some v"
-              by (metis fun_upd_apply get_state_set_state get_vh_def set_value_charact(2))
-            moreover have "snd (Rep_virtual_state (get_state (update_heap_val \<omega> l v))) la = Some v"
-              by (metis True fun_upd_apply get_state_set_state get_vh_def set_value_charact(2))
-            ultimately show ?thesis
-              by (metis True \<open>get_h \<omega>f l = None\<close> get_vh_def plus_option.simps(2))
-          next
-            case False
-            then have "Some (snd (Rep_virtual_state (get_state (update_heap_val \<omega>' l v))) la)
-  = Some (snd (Rep_virtual_state (get_state \<omega>')) la)"
-              by (metis fun_upd_apply get_state_set_state get_vh_def set_value_charact(2))
-            moreover have "snd (Rep_virtual_state (get_state (update_heap_val \<omega> l v))) la
-  = snd (Rep_virtual_state (get_state \<omega>)) la"
-              by (metis False fun_upd_apply get_state_set_state get_vh_def set_value_charact(2))
-            ultimately show ?thesis
-              by (metis assms(1) get_vh_def plus_funE state_add_iff vstate_add_iff)
-          qed
-        qed
-      qed
-    qed
+lemma sum_equi_states_easy:
+  fixes \<tau> :: "'a ag_trace"
+  assumes "Some \<omega> = a \<oplus> b"
+  shows "Some (Ag s, \<tau>, \<omega>) = (Ag s, \<tau>, a) \<oplus> (Ag s, \<tau>, b)"
+proof (rule plus_prodI)
+  show "Some (fst (Ag s, \<tau>, \<omega>)) = fst (Ag s, \<tau>, a) \<oplus> fst (Ag s, \<tau>, b)"
+    by (simp add: plus_AgI)
+  show "Some (snd (Ag s, \<tau>, \<omega>)) = snd (Ag s, \<tau>, a) \<oplus> snd (Ag s, \<tau>, b)"
+  proof (rule plus_prodI)
+    show "Some (fst (snd (Ag s, \<tau>, \<omega>))) = fst (snd (Ag s, \<tau>, a)) \<oplus> fst (snd (Ag s, \<tau>, b))"
+      by (simp add: plus_AgI)
+    show "Some (snd (snd (Ag s, \<tau>, \<omega>))) = snd (snd (Ag s, \<tau>, a)) \<oplus> snd (snd (Ag s, \<tau>, b))"
+      using assms by force
   qed
 qed
 
-
-definition full_ownership :: "var \<Rightarrow> int equi_state set"
-  where
-  "full_ownership r = { \<omega> |\<omega> l. get_store \<omega> r = Some (VRef (Address l)) \<and> get_m \<omega> (l, field_val) = 1}"
-
-definition full_ownership_with_val where
-  "full_ownership_with_val r e = { \<omega> |\<omega> l. get_store \<omega> r = Some (VRef (Address l)) \<and> get_m \<omega> (l, field_val) = 1
-  \<and> get_h \<omega> (l, field_val) = Some (VInt (edenot e (get_store \<omega>)))  }"
-
-lemma in_read_dom_write_dom:
-  assumes "get_m \<omega> (l, field_val) = 1"
-  shows "l \<in> read_dom \<omega>"
-    and "l \<in> write_dom \<omega>"
-  apply (metis CollectI assms not_gr_0 read_dom_def zero_neq_one)
-  by (simp add: assms write_dom_def)
-
-lemma stable_before_then_update_stable:
-  assumes "sep_algebra_class.stable \<omega>"
-      and "get_h \<omega> l \<noteq> None"
-  shows "sep_algebra_class.stable (update_heap_val \<omega> l v)"
+lemma sum_equi_states_easy_rev:
+  fixes \<tau> :: "'a ag_trace"
+  assumes "Some (Ag s, \<tau>, \<omega>) = (s1, \<tau>1, \<omega>1) \<oplus> (s2, \<tau>2, \<omega>2)"
+  shows "s1 = Ag s \<and> s2 = Ag s \<and> \<tau>1 = \<tau> \<and> \<tau>2 = \<tau> \<and> Some \<omega> = \<omega>1 \<oplus> \<omega>2"
   sorry
 
-proposition rule_write:
-  "CSL (full_ownership r) (Cwrite r e) (full_ownership_with_val r e)"
-proof (rule CSL_I)
-  fix n \<omega> assume "\<omega> \<in> full_ownership r" "sep_algebra_class.stable \<omega>"
-  then obtain l where asm0: "get_store \<omega> r = Some (VRef (Address l)) \<and> get_m \<omega> (l, field_val) = 1"
-    using full_ownership_def by blast
-  show "safe n (Cwrite r e) \<omega> (full_ownership_with_val r e)"
-  proof (cases n)
-    case (Suc m)
-    moreover have "safe (Suc m) (Cwrite r e) \<omega> (full_ownership_with_val r e)"
-    proof (rule safeI_alt)
-      have "accesses (Cwrite r e) (get_store \<omega>) = {l}" using get_address_simp asm0 by auto
-      then show "accesses (Cwrite r e) (get_store \<omega>) \<subseteq> read_dom \<omega>" using asm0
-        by (simp add: in_read_dom_write_dom(1))
-      show "writes (Cwrite r e) (get_store \<omega>) \<subseteq> write_dom \<omega>"
-        by (metis \<open>\<And>thesis. (\<And>l. get_store \<omega> r = Some (VRef (Address l)) \<and> get_m \<omega> (l, field_val) = PosReal.pwrite \<Longrightarrow> thesis) \<Longrightarrow> thesis\<close> get_address_simp in_read_dom_write_dom(2) singletonD subsetI writes.simps(4))
-      
-      fix \<omega>0' \<omega>f
-      assume asm1: "Some \<omega>0' = \<omega> \<oplus> \<omega>f \<and> binary_mask \<omega>0'" "sep_algebra_class.stable \<omega>f"
-      then have "get_store \<omega>0' r = Some (VRef (Address l)) \<and> get_m \<omega>0' (l, field_val) = 1"
-        by (metis asm0 binary_mask_def full_add_charact(1) get_m_additive padd_pos)
-      then have "get_h \<omega>0' (l, field_val) \<noteq> None"
-        by (simp add: pperm_pnone_pgt vstate_wf_imp)
+lemma frame_safe:
+  assumes "safe n C s \<tau> \<omega> Q"
+      and "fvA R \<inter> wrC C = {}"
+      and "Some \<omega>' = \<omega> \<oplus> \<omega>f"
+      and "(Ag s, \<tau>, \<omega>f) \<in> R"
+      and "sep_algebra_class.stable \<omega>f"
+    shows "safe n C s \<tau> \<omega>' (Q \<otimes> R)"
+  using assms
+proof (induct n arbitrary: C \<omega> \<omega>' \<omega>f s)
+  case (Suc n)
+  show ?case
+  proof (rule safeI)
+    show "C = Cskip \<Longrightarrow> (Ag s, \<tau>, \<omega>') \<in> Q \<otimes> R"
+      using safeE(1)[OF Suc(2)]
+      by (meson Suc.prems(3) Suc.prems(4) sum_equi_states_easy x_elem_set_product)
+    show "accesses C s \<subseteq> read_dom \<omega>'"
+      using safeE(2)[OF Suc(2)]
+      using Suc.prems(3) commutative greater_equiv read_dom_mono by fastforce
+    show "writes C s \<subseteq> write_dom \<omega>'"
+      by (metis (no_types, lifting) Suc.prems(1) Suc.prems(3) greater_def inf.absorb_iff2 inf.coboundedI1 safeE(3) write_dom_mono)
+    show "no_aborts C s \<omega>'"
+      by (meson Suc.prems(1) Suc.prems(3) greater_def no_aborts_mono safeE(4))
+    fix \<omega>0' \<omega>f' C' \<sigma>'
+    assume asm0: "sep_algebra_class.stable \<omega>f'" "Some \<omega>0' = \<omega>' \<oplus> \<omega>f'" "binary_mask \<omega>0'" "\<langle>C, concretize s \<omega>0'\<rangle> \<rightarrow> \<langle>C', \<sigma>'\<rangle>"
+    then obtain \<omega>f'' where "Some \<omega>f'' = \<omega>f \<oplus> \<omega>f'"
+      by (metis (no_types, opaque_lifting) Suc.prems(3) asso2 option.collapse)
+    then have "Some \<omega>0' = \<omega> \<oplus> \<omega>f''"
+      using asm0 Suc.prems(3) asso1 by force
+    then obtain \<omega>1'' \<omega>1' where "Some \<omega>1' = \<omega>1'' \<oplus> \<omega>f'' \<and> binary_mask \<omega>1' \<and> snd \<sigma>' = get_vh \<omega>1'" "safe n C' (fst \<sigma>') \<tau> \<omega>1'' Q"
+      "sep_algebra_class.stable \<omega>1''"
+      using safeE(5)[OF Suc(2), of \<omega>0' \<omega>f'' C' \<sigma>'] asm0 
+      by (meson Suc.prems(1) Suc.prems(5) \<open>Some \<omega>f'' = \<omega>f \<oplus> \<omega>f'\<close> safeE(5) stable_sum)
+    then obtain \<omega>1 where "Some \<omega>1 = \<omega>1'' \<oplus> \<omega>f"
+      by (metis (no_types, opaque_lifting) \<open>Some \<omega>f'' = \<omega>f \<oplus> \<omega>f'\<close> asso3 option.collapse)
+    moreover have "safe n C' (fst \<sigma>') \<tau> \<omega>1 (Q \<otimes> R)"
+      using \<open>safe n C' (fst \<sigma>') \<tau> \<omega>1'' Q\<close>
+    proof (rule Suc(1)[of C' _ \<omega>1'' \<omega>1 \<omega>f])
+      show "fvA R \<inter> wrC C' = {}"
+        by (meson Suc.prems(2) asm0 disjoint_iff red_properties subset_iff)
+      show "Some \<omega>1 = \<omega>1'' \<oplus> \<omega>f"
+        using calculation by auto
+      have "agrees (-(wrC C)) s (fst \<sigma>')"
+        by (metis agrees_search(1) asm0(4) fst_conv red_properties)
+      then have "agrees (fvA R) s (fst \<sigma>')"
+        using Suc.prems(2) agrees_search(3) by auto
+      then show "(Ag (fst \<sigma>'), \<tau>, \<omega>f) \<in> R"
+        by (meson Suc.prems(4) fvA_agrees)
+    qed (simp_all add: Suc.prems)
+    ultimately show "\<exists>\<omega>1 \<omega>1'. Some \<omega>1' = \<omega>1 \<oplus> \<omega>f' \<and> sep_algebra_class.stable \<omega>1 \<and> binary_mask \<omega>1' \<and> snd \<sigma>' = get_vh \<omega>1' \<and> safe n C' (fst \<sigma>') \<tau> \<omega>1 (Q \<otimes> R)"
+      by (metis Suc.prems(5) \<open>Some \<omega>1' = \<omega>1'' \<oplus> \<omega>f'' \<and> binary_mask \<omega>1' \<and> snd \<sigma>' = get_vh \<omega>1'\<close> \<open>Some \<omega>f'' = \<omega>f \<oplus> \<omega>f'\<close> \<open>sep_algebra_class.stable \<omega>1''\<close> asso1 stable_sum)
+  qed
+qed (simp)
 
-      show "aborts (Cwrite r e) (concretize \<omega>0') \<Longrightarrow> False"
-      proof -
-        assume "aborts (Cwrite r e) (concretize \<omega>0')"
-        then show False
-          using aborts_write_elim
-          using \<open>get_h \<omega>0' (l, field_val) \<noteq> None\<close> \<open>get_store \<omega>0' r = Some (VRef (Address l)) \<and> get_m \<omega>0' (l, field_val) = PosReal.pwrite\<close> concretize_def domIff fst_conv option.sel by auto
-      qed
-      fix C' \<sigma>'
-      assume asm2: "sep_algebra_class.stable \<omega>f" "\<langle>Cwrite r e, concretize \<omega>0'\<rangle> \<rightarrow> \<langle>C', \<sigma>'\<rangle>"
-      let ?v = "VInt (edenot e (get_store \<omega>0'))"
-
-      have "Some (update_heap_val \<omega>0' (l, field_val) ?v) = update_heap_val \<omega> (l, field_val) ?v \<oplus> \<omega>f"
-        using asm0 asm1 asm2 write_helper by blast
-      moreover have "\<sigma>' = concretize (update_heap_val \<omega>0' (l, field_val) ?v) \<and> C' = Cskip"
-        using red_write_cases[OF asm2(2)]
-        by (metis (no_types, lifting) \<open>get_store \<omega>0' r = Some (VRef (Address l)) \<and> get_m \<omega>0' (l, field_val) = PosReal.pwrite\<close> concretize_def get_state_set_state get_store_set_state old.prod.inject option.sel ref.sel set_value_charact(2) val.sel(4))
-      moreover have "safe m Cskip (update_heap_val \<omega> (l, field_val) ?v) (full_ownership_with_val r e)"
-      proof (rule safe_skip)
-        show "update_heap_val \<omega> (l, field_val) (VInt (edenot e (get_store \<omega>0'))) \<in> full_ownership_with_val r e"
-          by (simp add: asm0 asm1 full_add_charact(1) full_ownership_with_val_def)
-      qed
-      ultimately show "\<exists>\<omega>1 \<omega>1'. Some \<omega>1' = \<omega>1 \<oplus> \<omega>f \<and> sep_algebra_class.stable \<omega>1 \<and> binary_mask \<omega>1' \<and> \<sigma>' = concretize \<omega>1' \<and> safe m C' \<omega>1 (full_ownership_with_val r e)"
-        by (metis \<open>sep_algebra_class.stable \<omega>\<close> asm0 asm1(1) binary_mask_def get_state_set_state not_gr_0 one_neq_zero set_value_charact(1) stable_before_then_update_stable vstate_wf_imp)
-    qed (simp)
-    ultimately show ?thesis by blast
-  qed (simp)
+(*
+lemma self_framing_wf_split:
+  assumes "\<omega> \<in> A \<otimes> B"
+      and "TypedEqui.wf_assertion \<Delta> A"
+      and "self_framing B"
+    shows "\<exists>a b. a \<in> A \<and> b \<in> B \<and> Some \<omega> = a \<oplus> b \<and> sep_algebra_class.stable b"
+proof -
+  obtain a b where "Some \<omega> = a \<oplus> b" "a \<in> A" "b \<in> B"
+    by (meson assms(1) x_elem_set_product)
+  then obtain a' where "Some a' = a \<oplus> |\<omega>|"
+    by (metis commutative minus_equiv_def_any_elem)
+  then have "Some \<omega> = a' \<oplus> stabilize b"
+    by (smt (verit, best) \<open>Some \<omega> = a \<oplus> b\<close> asso1 commutative core_is_pure core_is_smaller core_sum decompose_stabilize_pure)
+  then show ?thesis
+    by (metis (no_types, opaque_lifting) TypedEqui.wf_assertion_def \<open>Some a' = a \<oplus> |\<omega>|\<close> \<open>a \<in> A\<close> \<open>b \<in> B\<close> assms(2) assms(3) core_is_pure in_Stabilize pure_def pure_larger_def self_framing_eq stabilize_is_stable)
 qed
+*)
+
+lemma sum_equi_states_easy_decompose:
+  fixes \<tau> :: "'a ag_trace"
+  assumes "(Ag s, \<tau>, \<omega>) \<in> P \<otimes> R"
+  shows "\<exists>\<omega>p \<omega>r. Some \<omega> = \<omega>p \<oplus> \<omega>r \<and> (Ag s, \<tau>, \<omega>p) \<in> P \<and> (Ag s, \<tau>, \<omega>r) \<in> R"
+  sorry
+
+lemma stabilize_equi_state:
+  fixes \<tau> :: "'a ag_trace"
+  shows "stabilize (Ag s, \<tau>, \<omega>) = (Ag s, \<tau>, stabilize \<omega>)"
+  by (smt (z3) core_def decompose_stabilize_pure snd_conv stabilize_prod_def sum_equi_states_easy_rev)
+
+
+proposition frame_rule:
+  assumes "CSL P C Q"
+      and "disjoint (fvA R) (wrC C)"
+      and "self_framing P"
+      and "self_framing R"
+    shows "CSL (P \<otimes> R) C (Q \<otimes> R)"
+proof (rule CSL_I)
+  fix n s \<tau> \<omega> assume "(Ag s, \<tau>, \<omega>) \<in> P \<otimes> R" "sep_algebra_class.stable \<omega>"
+  then obtain \<omega>p \<omega>r where r: "Some \<omega> = \<omega>p \<oplus> \<omega>r" "(Ag s, \<tau>, \<omega>p) \<in> P" "(Ag s, \<tau>, \<omega>r) \<in> R"
+    by (meson sum_equi_states_easy_decompose)
+  then have "Some \<omega> = stabilize \<omega>p \<oplus> stabilize \<omega>r"
+    using \<open>sep_algebra_class.stable \<omega>\<close> stabilize_sum_of_stable by blast
+  then show "safe (Suc n) C s \<tau> \<omega> (Q \<otimes> R)"
+    using frame_safe[of n C s \<tau> "stabilize \<omega>p" Q R \<omega> "stabilize \<omega>r"]
+    by (metis (no_types, lifting) CSL_def assms(1) assms(2) assms(3) assms(4) disjoint_def frame_safe r(2) r(3) self_framing_def stabilize_equi_state stabilize_is_stable)
+qed
+
+
 
 
 subsection \<open>Parallel rule\<close>
@@ -491,84 +386,94 @@ lemma write_dom_union:
   sorry
 
 lemma safe_par:
-  assumes "safe n C1 \<omega>1 Q1"
-      and "safe n C2 \<omega>2 Q2"
+  assumes "safe n C1 s \<tau> \<omega>1 Q1"
+      and "safe n C2 s \<tau> \<omega>2 Q2"
       and "Some \<omega> = \<omega>1 \<oplus> \<omega>2"
       and "disjoint (fvC C1 \<union> fvA Q1) (wrC C2)"
       and "disjoint (fvC C2 \<union> fvA Q2) (wrC C1)"
       and "sep_algebra_class.stable \<omega>1"
       and "sep_algebra_class.stable \<omega>2"
-    shows "safe n (C1 || C2) \<omega> (Q1 \<otimes> Q2)"
+    shows "safe n (C1 || C2) s \<tau> \<omega> (Q1 \<otimes> Q2)"
   using assms
-proof (induct n arbitrary: C1 C2 \<omega>1 \<omega>2 \<omega>)
+proof (induct n arbitrary: C1 C2 \<omega>1 \<omega>2 \<omega> s)
   case (Suc n)
-  show "safe (Suc n) (C1 || C2) \<omega> (Q1 \<otimes> Q2)"
+  show "safe (Suc n) (C1 || C2) s \<tau> \<omega> (Q1 \<otimes> Q2)"
   proof (rule safeI_alt)
-    show "accesses (C1 || C2) (get_store \<omega>) \<subseteq> read_dom \<omega>"
-      by (metis Suc.prems(1) Suc.prems(2) Suc.prems(3) Un_mono accesses.simps(8) full_add_charact(1) full_add_defined read_dom_union safeE(2))
-    show "writes (C1 || C2) (get_store \<omega>) \<subseteq> write_dom \<omega>"
+    show "accesses (C1 || C2) s \<subseteq> read_dom \<omega>"
+      by (metis Suc.prems(1) Suc.prems(2) Suc.prems(3) Un_mono accesses.simps(8) read_dom_union safeE(2))
+    show "writes (C1 || C2) s \<subseteq> write_dom \<omega>"
     proof -
-      have "writes C1 (get_store \<omega>) \<subseteq> write_dom \<omega> \<and> writes C2 (get_store \<omega>) \<subseteq> write_dom \<omega>"
-        by (metis (no_types, lifting) Suc.prems(1) Suc.prems(2) Suc.prems(3) commutative dual_order.trans full_add_charact(1) le_supE safeE(3) write_dom_union)
+      have "writes C1 s \<subseteq> write_dom \<omega> \<and> writes C2 s \<subseteq> write_dom \<omega>"
+        by (metis (no_types, lifting) Suc.prems(1) Suc.prems(2) Suc.prems(3) dual_order.trans le_supE safeE(3) write_dom_union)
       then show ?thesis
         by simp
     qed
     fix \<omega>0' \<omega>f
-    assume asm0: "sep_algebra_class.stable \<omega>f" "Some \<omega>0' = \<omega> \<oplus> \<omega>f \<and> binary_mask \<omega>0'"
-    show "aborts (C1 || C2) (concretize \<omega>0') \<Longrightarrow> False"
+    assume asm0: "sep_algebra_class.stable \<omega>f" "Some \<omega>0' = \<omega> \<oplus> \<omega>f" "binary_mask \<omega>0'"
+    show "aborts (C1 || C2) (concretize s \<omega>0') \<Longrightarrow> False"
     proof -
-      assume "aborts (C1 || C2) (concretize \<omega>0')"
+      assume "aborts (C1 || C2) (concretize s \<omega>0')"
       then show "False"
       proof (rule aborts_par_elim)
-        show "aborts C1 (concretize \<omega>0') \<Longrightarrow> False"
-          using Suc.prems(1) Suc.prems(3) asm0(1) asm0(2) greater_def no_aborts_def no_aborts_mono safe.simps(2) by blast
-        show "aborts C2 (concretize \<omega>0') \<Longrightarrow> False"
-          using Suc.prems(2) Suc.prems(3) asm0(1) asm0(2) greater_def no_aborts_def no_aborts_mono safe.simps(2)
+        show "aborts C1 (concretize s \<omega>0') \<Longrightarrow> False"
+          using safeE(4)[OF Suc.prems(1)]
+          using Suc.prems(3) asm0 greater_def no_aborts_def no_aborts_mono by blast
+        show "aborts C2 (concretize s \<omega>0') \<Longrightarrow> False"
+          using Suc.prems(2) Suc.prems(3) asm0 greater_def no_aborts_def no_aborts_mono safe.simps(2)
           by (metis commutative)
-        have r1: "accesses C1 (fst (concretize \<omega>1)) \<subseteq> read_dom \<omega>1 \<and> writes C1 (fst (concretize \<omega>1)) \<subseteq> write_dom \<omega>1"
-          using Suc.prems(1) concretize_def by auto
-        moreover have r2: "accesses C2 (fst (concretize \<omega>2)) \<subseteq> read_dom \<omega>2 \<and> writes C2 (fst (concretize \<omega>2)) \<subseteq> write_dom \<omega>2"
-          using Suc.prems(2) concretize_def by auto
-        ultimately show "\<not> disjoint (accesses C1 (fst (concretize \<omega>0'))) (writes C2 (fst (concretize \<omega>0'))) \<Longrightarrow> False"
-          by (metis (no_types, lifting) Pair_inject Suc.prems(3) asm0(2) commutative concretize_def defined_def disj_conv disjoint_search(3) disjoint_search(4) full_add_charact(1) option.simps(3) prod.exhaust_sel)
-        show "\<not> disjoint (writes C1 (fst (concretize \<omega>0'))) (accesses C2 (fst (concretize \<omega>0'))) \<Longrightarrow> False"
-          by (metis (no_types, lifting) Pair_inject Suc.prems(3) asm0(2) concretize_def defined_def disj_conv disjoint_search(5) full_add_charact(1) full_add_defined option.discI r1 r2 surjective_pairing)
+        have r1: "accesses C1 s \<subseteq> read_dom \<omega>1 \<and> writes C1 s \<subseteq> write_dom \<omega>1"
+          using Suc.prems(1) by auto
+        moreover have r2: "accesses C2 s \<subseteq> read_dom \<omega>2 \<and> writes C2 s \<subseteq> write_dom \<omega>2"
+          using Suc.prems(2) by auto
+        ultimately show "\<not> disjoint (accesses C1 (fst (concretize s \<omega>0'))) (writes C2 (fst (concretize s \<omega>0'))) \<Longrightarrow> False"
+          by (metis (no_types, lifting) Pair_inject Suc.prems(3) commutative defined_def disj_conv disjoint_search(3) disjoint_search(4) option.simps(3) prod.exhaust_sel)
+        show "\<not> disjoint (writes C1 (fst (concretize s \<omega>0'))) (accesses C2 (fst (concretize s \<omega>0'))) \<Longrightarrow> False"
+          by (metis (no_types, lifting) Pair_inject Suc.prems(3) defined_def disj_conv disjoint_search(5) option.discI r1 r2 surjective_pairing)
       qed
     qed
 
     fix C' \<sigma>'
-    assume asm1: "\<langle>C1 || C2, concretize \<omega>0'\<rangle> \<rightarrow> \<langle>C', \<sigma>'\<rangle>"
-    then show "\<exists>\<omega>1 \<omega>1'. Some \<omega>1' = \<omega>1 \<oplus> \<omega>f \<and> sep_algebra_class.stable \<omega>1 \<and> binary_mask \<omega>1' \<and> \<sigma>' = concretize \<omega>1' \<and> safe n C' \<omega>1 (Q1 \<otimes> Q2)"
+    assume asm1: "\<langle>C1 || C2, concretize s \<omega>0'\<rangle> \<rightarrow> \<langle>C', \<sigma>'\<rangle>"
+    then show "\<exists>\<omega>1 \<omega>1'. Some \<omega>1' = \<omega>1 \<oplus> \<omega>f \<and> sep_algebra_class.stable \<omega>1 \<and> binary_mask \<omega>1' \<and> snd \<sigma>' = get_vh \<omega>1' \<and> safe n C' (fst \<sigma>') \<tau> \<omega>1 (Q1 \<otimes> Q2)"
     proof (rule red_par_cases)
-      show "C' = Cskip \<Longrightarrow> \<sigma>' = concretize \<omega>0' \<Longrightarrow> C1 = Cskip \<Longrightarrow> C2 = Cskip
-  \<Longrightarrow> \<exists>\<omega>1 \<omega>1'. Some \<omega>1' = \<omega>1 \<oplus> \<omega>f \<and> sep_algebra_class.stable \<omega>1 \<and> binary_mask \<omega>1' \<and> \<sigma>' = concretize \<omega>1' \<and> safe n C' \<omega>1 (Q1 \<otimes> Q2)"
-        by (metis (no_types, lifting) Suc.prems(1) Suc.prems(2) Suc.prems(3) Suc.prems(6) Suc.prems(7) asm0(2) is_in_set_sum safeE(1) safe_skip stable_sum star_to_singletonI)
+      show "C' = Cskip \<Longrightarrow> \<sigma>' = concretize s \<omega>0' \<Longrightarrow> C1 = Cskip \<Longrightarrow> C2 = Cskip
+  \<Longrightarrow> \<exists>\<omega>1 \<omega>1'. Some \<omega>1' = \<omega>1 \<oplus> \<omega>f \<and> sep_algebra_class.stable \<omega>1 \<and> binary_mask \<omega>1' \<and> snd \<sigma>' = get_vh \<omega>1' \<and> safe n C' (fst \<sigma>') \<tau> \<omega>1 (Q1 \<otimes> Q2)"
+        using safeE(1)[OF Suc.prems(1)] safeE(1)[OF Suc.prems(2)]
+        by (metis Suc.prems(3) Suc.prems(5) Suc.prems(6) Suc.prems(7) asm0(2) asm0(3) disjoint_def disjoint_simps(3) frame_safe fst_conv safe_skip snd_conv stable_sum)
       fix C1'
-      assume asm2: "C' = C1' || C2" "\<langle>C1, concretize \<omega>0'\<rangle> \<rightarrow> \<langle>C1', \<sigma>'\<rangle>"
+      assume asm2: "C' = C1' || C2" "\<langle>C1, concretize s \<omega>0'\<rangle> \<rightarrow> \<langle>C1', \<sigma>'\<rangle>"
       obtain \<omega>f' where "Some \<omega>f' = \<omega>2 \<oplus> \<omega>f"
         by (metis (no_types, opaque_lifting) Suc.prems(3) asm0(2) asso2 option.exhaust_sel)
       then have "Some \<omega>0' = \<omega>1 \<oplus> \<omega>f'"
         using Suc.prems(3) asm0(2) asso1 by force
-      then obtain \<omega>a \<omega>a' where ra: "Some \<omega>a' = \<omega>a \<oplus> \<omega>f' \<and> binary_mask \<omega>a' \<and> \<sigma>' = concretize \<omega>a'" "safe n C1' \<omega>a Q1"
+      then obtain \<omega>a \<omega>a' where ra: "Some \<omega>a' = \<omega>a \<oplus> \<omega>f' \<and> binary_mask \<omega>a' \<and> snd \<sigma>' = get_vh \<omega>a'" "safe n C1' (fst \<sigma>') \<tau> \<omega>a Q1"
         "sep_algebra_class.stable \<omega>a"
         using safeE(5)[OF Suc(2), of \<omega>f' \<omega>0' C1' \<sigma>'] asm0 asm2(2)
         using Suc.prems(7) \<open>Some \<omega>f' = \<omega>2 \<oplus> \<omega>f\<close> stable_sum by blast
-      moreover have "safe n C2 \<omega>2 Q2"
-        by (meson Suc.prems(2) Suc_n_not_le_n nat_le_linear safety_mono)
+      moreover have "safe n C2 (fst \<sigma>') \<tau> \<omega>2 Q2"
+      proof -
+        have "safe n C2 s \<tau> \<omega>2 Q2"
+          by (meson Suc.prems(2) Suc_n_not_le_n nat_le_linear safety_mono)
+        moreover have "agrees (-wrC C1) s (fst \<sigma>')"
+          by (metis agrees_search(1) asm2(2) fst_conv red_properties)
+        ultimately show ?thesis
+          using Suc.prems(5) agrees_minusD disjoint_commute safe_agrees by blast
+      qed
       moreover obtain \<omega>' where "Some \<omega>' = \<omega>a \<oplus> \<omega>2"
         by (metis (no_types, opaque_lifting) \<open>Some \<omega>f' = \<omega>2 \<oplus> \<omega>f\<close> asso2 calculation(1) commutative option.exhaust_sel)
       then have "Some \<omega>a' = \<omega>' \<oplus> \<omega>f"
         by (metis \<open>Some \<omega>f' = \<omega>2 \<oplus> \<omega>f\<close> asso1 calculation(1))
-      ultimately have "safe n C' \<omega>' (Q1 \<otimes> Q2)"
-        using Suc(1)[OF ra(2) \<open>safe n C2 \<omega>2 Q2\<close>]
+      ultimately have "safe n C' (fst \<sigma>') \<tau> \<omega>' (Q1 \<otimes> Q2)"
+        using Suc(1)[OF ra(2) \<open>safe n C2 (fst \<sigma>') \<tau> \<omega>2 Q2\<close>]
         by (metis (no_types, lifting) Suc.prems(4) Suc.prems(5) Suc.prems(7) \<open>Some \<omega>' = \<omega>a \<oplus> \<omega>2\<close> asm2(1) asm2(2) disjoint_search(2) disjoint_search(4) disjoint_simps(3) red_properties)
-      then show "\<exists>\<omega>1 \<omega>1'. Some \<omega>1' = \<omega>1 \<oplus> \<omega>f \<and> sep_algebra_class.stable \<omega>1 \<and> binary_mask \<omega>1' \<and> \<sigma>' = concretize \<omega>1' \<and> safe n C' \<omega>1 (Q1 \<otimes> Q2)"
+      
+      then show "\<exists>\<omega>1 \<omega>1'. Some \<omega>1' = \<omega>1 \<oplus> \<omega>f \<and> sep_algebra_class.stable \<omega>1 \<and> binary_mask \<omega>1' \<and> snd \<sigma>' = get_vh \<omega>1' \<and> safe n C' (fst \<sigma>') \<tau> \<omega>1 (Q1 \<otimes> Q2)"
         using \<open>Some \<omega>a' = \<omega>' \<oplus> \<omega>f\<close> ra(1)
         using Suc.prems(7) \<open>Some \<omega>' = \<omega>a \<oplus> \<omega>2\<close> \<open>sep_algebra_class.stable \<omega>a\<close> stable_sum by blast
     next
       show "\<And>C2'. C' = C1 || C2' \<Longrightarrow>
-           \<langle>C2, concretize \<omega>0'\<rangle> \<rightarrow> \<langle>C2', \<sigma>'\<rangle> \<Longrightarrow>
-           \<exists>\<omega>1 \<omega>1'. Some \<omega>1' = \<omega>1 \<oplus> \<omega>f \<and> sep_algebra_class.stable \<omega>1 \<and> binary_mask \<omega>1' \<and> \<sigma>' = concretize \<omega>1' \<and> safe n C' \<omega>1 (Q1 \<otimes> Q2)"
+           \<langle>C2, concretize s \<omega>0'\<rangle> \<rightarrow> \<langle>C2', \<sigma>'\<rangle> \<Longrightarrow>
+           \<exists>\<omega>1 \<omega>1'. Some \<omega>1' = \<omega>1 \<oplus> \<omega>f \<and> sep_algebra_class.stable \<omega>1 \<and> binary_mask \<omega>1' \<and> snd \<sigma>' = get_vh \<omega>1' \<and> safe n C' (fst \<sigma>') \<tau> \<omega>1 (Q1 \<otimes> Q2)"
         sorry
 (* TODO: same proof *)
     qed
@@ -587,15 +492,690 @@ proposition rule_par:
       and "self_framing P2"
     shows "CSL (P1 \<otimes> P2) (C1 || C2) (Q1 \<otimes> Q2)"
 proof (rule CSL_I)
-  fix n \<omega>
-  assume asm0: "\<omega> \<in> P1 \<otimes> P2" "sep_algebra_class.stable \<omega>"
-  then obtain p1 p2 where "Some \<omega> = p1 \<oplus> p2" "p1 \<in> P1" "p2 \<in> P2"
-    by (meson x_elem_set_product)
+  fix n s \<tau> \<omega>
+  assume asm0: "(Ag s, \<tau>, \<omega>) \<in> P1 \<otimes> P2" "sep_algebra_class.stable \<omega>"
+  then obtain p1 p2 where "Some \<omega> = p1 \<oplus> p2" "(Ag s, \<tau>, p1) \<in> P1" "(Ag s, \<tau>, p2) \<in> P2"
+    by (meson sum_equi_states_easy_decompose)
   then have "Some \<omega> = stabilize p1 \<oplus> stabilize p2"
     using asm0(2) stabilize_sum_of_stable by blast
-  then show "safe n (C1 || C2) \<omega> (Q1 \<otimes> Q2)"
-    by (meson CSL_def \<open>\<And>thesis. (\<And>p1 p2. \<lbrakk>Some \<omega> = p1 \<oplus> p2; p1 \<in> P1; p2 \<in> P2\<rbrakk> \<Longrightarrow> thesis) \<Longrightarrow> thesis\<close> asm0(2) assms(1) assms(2) assms(3) assms(4) assms(5) assms(6) safe_par self_framing_def stabilize_is_stable stabilize_sum_of_stable)
+  then show "safe (Suc n) (C1 || C2) s \<tau> \<omega> (Q1 \<otimes> Q2)"
+    using safe_par[of "Suc n" C1 s \<tau> p1 Q1 C2 p2 Q2 \<omega>]
+    by (metis CSL_def \<open>(Ag s, \<tau>, p1) \<in> P1\<close> \<open>(Ag s, \<tau>, p2) \<in> P2\<close> assms(1) assms(2) assms(3) assms(4) assms(5) assms(6) safe_par self_framing_def stabilize_equi_state stabilize_is_stable)
 qed
+
+
+subsection \<open>Sequential composition\<close>
+
+lemma safe_seq:
+  assumes "safe n C1 s \<tau> \<omega> Q"
+      and "\<And>m \<omega>' s'. m \<le> n \<and> (Ag s', \<tau>, \<omega>') \<in> Q \<and> sep_algebra_class.stable \<omega>' \<Longrightarrow> safe m C2 s' \<tau> \<omega>' R"
+      and "sep_algebra_class.stable \<omega>"
+    shows "safe n (Cseq C1 C2) s \<tau> \<omega> R"
+  using assms
+proof (induct n arbitrary: C1 \<omega> s)
+  case (Suc n)
+  show "safe (Suc n) (Cseq C1 C2) s \<tau> \<omega> R"
+  proof (rule safeI)
+    show "accesses (Cseq C1 C2) s \<subseteq> read_dom \<omega>"
+      using Suc.prems(1) accesses.simps(7) safeE(2) by blast
+    show "writes (Cseq C1 C2) s \<subseteq> write_dom \<omega>"
+      by (metis Suc.prems(1) safeE(3) writes.simps(7))
+    show "no_aborts (Cseq C1 C2) s \<omega>"
+      using safeE(4)[OF Suc.prems(1)] aborts_seq_elim
+      by (meson no_aborts_def)
+    fix \<omega>0' \<omega>f C' \<sigma>'
+    assume asm0: "sep_algebra_class.stable \<omega>f" "Some \<omega>0' = \<omega> \<oplus> \<omega>f" "binary_mask \<omega>0'"
+    assume "\<langle>Cseq C1 C2, concretize s \<omega>0'\<rangle> \<rightarrow> \<langle>C', \<sigma>'\<rangle>"
+    then show "\<exists>\<omega>1 \<omega>1'. Some \<omega>1' = \<omega>1 \<oplus> \<omega>f \<and> sep_algebra_class.stable \<omega>1 \<and> binary_mask \<omega>1' \<and> snd \<sigma>' = get_vh \<omega>1' \<and> safe n C' (fst \<sigma>') \<tau> \<omega>1 R"
+    proof (rule red_seq_cases)
+      assume asm1: "C1 = Cskip" "C' = C2" "\<sigma>' = concretize s \<omega>0'"
+      then have "safe (Suc n) C2 s \<tau> \<omega> R"
+        using Suc.prems(2)[of "Suc n" _ \<omega>] safeE(1)[OF Suc.prems(1)] Suc.prems(3) by blast
+      then show "\<exists>\<omega>1 \<omega>1'. Some \<omega>1' = \<omega>1 \<oplus> \<omega>f \<and> sep_algebra_class.stable \<omega>1 \<and> binary_mask \<omega>1' \<and> snd \<sigma>' = get_vh \<omega>1' \<and> safe n C' (fst \<sigma>') \<tau> \<omega>1 R"
+        using safeE(5)
+        by (metis (no_types, lifting) Suc.prems(3) Suc_n_not_le_n asm0(2) asm0(3) asm1(2) asm1(3) fst_conv nat_le_linear safety_mono snd_conv)
+    next
+      fix C1' assume asm1: "C' = Cseq C1' C2" "\<langle>C1, concretize s \<omega>0'\<rangle> \<rightarrow> \<langle>C1', \<sigma>'\<rangle>"
+      then obtain \<omega>1 \<omega>1' where "Some \<omega>1' = \<omega>1 \<oplus> \<omega>f" "sep_algebra_class.stable \<omega>1" "binary_mask \<omega>1'"
+        "snd \<sigma>' = get_vh \<omega>1'" "safe n C1' (fst \<sigma>') \<tau> \<omega>1 Q"
+        using safeE(5)[OF Suc.prems(1), of \<omega>f \<omega>0' C1' \<sigma>'] asm0(1) asm0(2) asm0(3) by blast
+      then have "safe n (Cseq C1' C2) (fst \<sigma>') \<tau> \<omega>1 R" using Suc(1)[OF \<open>safe n C1' (fst \<sigma>') \<tau> \<omega>1 Q\<close>]
+        by (simp add: Suc.prems(2))
+      then show "\<exists>\<omega>1 \<omega>1'. Some \<omega>1' = \<omega>1 \<oplus> \<omega>f \<and> sep_algebra_class.stable \<omega>1 \<and> binary_mask \<omega>1' \<and> snd \<sigma>' = get_vh \<omega>1' \<and> safe n C' (fst \<sigma>') \<tau> \<omega>1 R"
+        using \<open>Some \<omega>1' = \<omega>1 \<oplus> \<omega>f\<close> \<open>binary_mask \<omega>1'\<close> \<open>sep_algebra_class.stable \<omega>1\<close> \<open>snd \<sigma>' = get_vh \<omega>1'\<close> asm1(1) by blast
+    qed
+  qed (simp)
+qed (simp)
+
+
+proposition rule_seq:
+  assumes "CSL P C1 Q"
+    and "CSL Q C2 R"
+    shows "CSL P (Cseq C1 C2) R"
+proof (rule CSL_I)
+  fix n s \<tau> \<omega>
+  assume asm0: "(Ag s, \<tau>, \<omega>) \<in> P" "sep_algebra_class.stable \<omega>"
+  show "safe n (Cseq C1 C2) s \<tau> \<omega> R"
+  proof (rule safe_seq[of n C1 s \<tau> \<omega> Q C2 R])
+    show "safe n C1 s \<tau> \<omega> Q"
+      using CSL_E asm0(1) asm0(2) assms(1) by blast
+    show "\<And>m \<omega>' s'. m \<le> n \<and> (Ag s', \<tau>, \<omega>') \<in> Q \<and> sep_algebra_class.stable \<omega>' \<Longrightarrow> safe m C2 s' \<tau> \<omega>' R"
+      using CSL_E[OF assms(2)] by blast
+  qed (simp add: asm0)
+qed
+
+
+
+subsection \<open>Consequence rule\<close>
+
+lemma safe_conseq:
+  assumes "safe n C s \<tau> \<omega> Q"
+      and "Q \<subseteq> Q'"
+    shows "safe n C s \<tau> \<omega> Q'"
+  using assms
+proof (induct n arbitrary: C \<omega> s)
+  case (Suc n)
+  show "safe (Suc n) C s \<tau> \<omega> Q'"
+  proof (rule safeI)
+    show "C = Cskip \<Longrightarrow> (Ag s, \<tau>, \<omega>) \<in> Q'"
+      using Suc.prems(1) assms(2) safe.simps(2) by blast
+    show "accesses C s \<subseteq> read_dom \<omega>"
+      using Suc.prems(1) safeE(2) by blast
+    show "writes C s \<subseteq> write_dom \<omega>"
+      using Suc.prems(1) by auto
+    show "no_aborts C s \<omega>"
+      using Suc.prems(1) safe.simps(2) by blast
+    fix \<omega>0' \<omega>f C' \<sigma>'
+    assume asm0: "sep_algebra_class.stable \<omega>f" "Some \<omega>0' = \<omega> \<oplus> \<omega>f" "binary_mask \<omega>0'"
+      "\<langle>C, concretize s \<omega>0'\<rangle> \<rightarrow> \<langle>C', \<sigma>'\<rangle>"
+    then show "\<exists>\<omega>1 \<omega>1'. Some \<omega>1' = \<omega>1 \<oplus> \<omega>f \<and> sep_algebra_class.stable \<omega>1 \<and> binary_mask \<omega>1' \<and> snd \<sigma>' = get_vh \<omega>1' \<and> safe n C' (fst \<sigma>') \<tau> \<omega>1 Q'"
+      using safeE(5)[OF Suc.prems(1)] by (meson Suc.hyps assms(2))
+  qed
+qed (simp)
+
+proposition rule_conseq:
+  assumes "CSL P C Q"
+      and "P' \<subseteq> P"
+      and "Q \<subseteq> Q'"
+    shows "CSL P' C Q'"
+proof (rule CSL_I)
+  show "\<And>n s \<tau> \<omega>. (Ag s, \<tau>, \<omega>) \<in> P' \<Longrightarrow> sep_algebra_class.stable \<omega> \<Longrightarrow> safe (Suc n) C s \<tau> \<omega> Q'"
+    using CSL_E assms(1) assms(2) assms(3) safe_conseq by blast
+qed
+
+
+
+subsection \<open>Conditional rule\<close>
+
+(*
+| RuleIf: "\<lbrakk> self_framing_and_typed \<Delta> A; framed_by_exp A b; \<Delta> \<turnstile> [A \<otimes> pure_typed \<Delta> b] C1 [B1] ; \<Delta> \<turnstile> [A \<otimes> pure_typed \<Delta> (negate b)] C2 [B2] \<rbrakk>
+  \<Longrightarrow> \<Delta> \<turnstile> [A] If b C1 C2 [B1 \<union> B2]"
+*)
+definition assertify_bexp where
+  "assertify_bexp b = { \<omega> |\<omega>. bdenot b (get_store \<omega>)}"
+
+lemma in_assertify_bexp:
+  assumes "bdenot b (get_store \<omega>)"
+  shows "\<omega> \<in> assertify_bexp b"
+  by (simp add: assertify_bexp_def assms)
+
+lemma in_assertify_bexp_alt:
+  assumes "bdenot b s"
+  shows "(Ag s, \<tau>, \<omega>) \<in> assertify_bexp b"
+  by (simp add: assms get_store_def in_assertify_bexp)
+
+proposition rule_if:
+  assumes "CSL (P \<inter> assertify_bexp b) C1 Q"
+      and "CSL (P \<inter> assertify_bexp (Bnot b)) C2 Q"
+    shows "CSL P (Cif b C1 C2) Q"
+proof (rule CSL_I)
+  fix n s \<tau> \<omega>
+  assume asm0: "(Ag s, \<tau>, \<omega>) \<in> P" "sep_algebra_class.stable \<omega>"
+  show "safe (Suc n) (Cif b C1 C2) s \<tau> \<omega> Q"
+  proof (rule safeI)
+    show "no_aborts (Cif b C1 C2) s \<omega>"
+      using aborts.cases cmd.distinct(45) cmd.distinct(57) cmd.distinct(85) cmd.simps(91) no_aborts_def by blast
+    fix \<omega>0' \<omega>f C' \<sigma>'
+    assume asm1: "sep_algebra_class.stable \<omega>f" "Some \<omega>0' = \<omega> \<oplus> \<omega>f" "binary_mask \<omega>0'"
+    assume "\<langle>Cif b C1 C2, concretize s \<omega>0'\<rangle> \<rightarrow> \<langle>C', \<sigma>'\<rangle>"
+    then show "\<exists>\<omega>1 \<omega>1'. Some \<omega>1' = \<omega>1 \<oplus> \<omega>f \<and> sep_algebra_class.stable \<omega>1 \<and> binary_mask \<omega>1' \<and> snd \<sigma>' = get_vh \<omega>1' \<and> safe n C' (fst \<sigma>') \<tau> \<omega>1 Q"
+    proof (rule red_if_cases)
+      assume asm2: "C' = C1" "\<sigma>' = concretize s \<omega>0'" "bdenot b (fst (concretize s \<omega>0'))"
+      then have "(Ag s, \<tau>, \<omega>) \<in> P \<inter> assertify_bexp b"
+        by (simp add: asm0(1) asm1(2) full_add_charact(1) in_assertify_bexp_alt)
+      then have "safe n C' s \<tau> \<omega> Q"
+        using CSL_E[OF assms(1), of s \<tau> \<omega> n] asm0 asm2 by blast
+      then show "\<exists>\<omega>1 \<omega>1'. Some \<omega>1' = \<omega>1 \<oplus> \<omega>f \<and> sep_algebra_class.stable \<omega>1 \<and> binary_mask \<omega>1' \<and> snd \<sigma>' = get_vh \<omega>1' \<and> safe n C' (fst \<sigma>') \<tau> \<omega>1 Q"
+        using asm0 asm1 asm2 by auto
+    next
+      assume asm2: "C' = C2" "\<sigma>' = concretize s \<omega>0'" "\<not> bdenot b (fst (concretize s \<omega>0'))"
+      then have "(Ag s, \<tau>, \<omega>) \<in> P \<inter> assertify_bexp (Bnot b)"
+        by (simp add: asm0(1) asm1(2) full_add_charact(1) in_assertify_bexp_alt)
+      then have "safe n C' s \<tau> \<omega> Q"
+        using CSL_E[OF assms(2), of s \<tau> \<omega> n] asm0 asm2 by blast
+      then show "\<exists>\<omega>1 \<omega>1'. Some \<omega>1' = \<omega>1 \<oplus> \<omega>f \<and> sep_algebra_class.stable \<omega>1 \<and> binary_mask \<omega>1' \<and> snd \<sigma>' = get_vh \<omega>1' \<and> safe n C' (fst \<sigma>') \<tau> \<omega>1 Q"
+        using asm0 asm1 asm2 by auto
+    qed
+  qed (simp_all)
+qed
+
+
+subsection \<open>While loops\<close>
+
+
+lemma safe_while:
+  assumes "CSL (I \<inter> (assertify_bexp b)) C I"
+      and "(Ag s, \<tau>, \<omega>) \<in> I"
+      and "sep_algebra_class.stable \<omega>"
+    shows "safe n (Cwhile b C) s \<tau> \<omega> (I \<inter> (assertify_bexp (Bnot b)))"
+  using assms
+proof (induct n arbitrary: \<omega> s)
+  case (Suc n)
+  note SucOuter = Suc
+  show "safe (Suc n) (Cwhile b C) s \<tau> \<omega> (I \<inter> assertify_bexp (Bnot b))"
+  proof (rule safeI)
+    show "no_aborts (Cwhile b C) s \<omega>"
+      using aborts_while_elim no_aborts_def by blast
+    fix \<omega>0' \<omega>f C' \<sigma>'
+    assume asm0: "sep_algebra_class.stable \<omega>f" "Some \<omega>0' = \<omega> \<oplus> \<omega>f" "binary_mask \<omega>0'"
+    assume "\<langle>Cwhile b C, concretize s \<omega>0'\<rangle> \<rightarrow> \<langle>C', \<sigma>'\<rangle>"
+    then show "\<exists>\<omega>1 \<omega>1'. Some \<omega>1' = \<omega>1 \<oplus> \<omega>f \<and> sep_algebra_class.stable \<omega>1 \<and> binary_mask \<omega>1' \<and> snd \<sigma>' = get_vh \<omega>1' \<and> safe n C' (fst \<sigma>') \<tau> \<omega>1 (I \<inter> assertify_bexp (Bnot b))"
+    proof (rule red_while_cases)
+      assume asm1: "C' = Cif b (Cseq C (Cwhile b C)) Cskip" "\<sigma>' = concretize s \<omega>0'"
+      have "safe n C' s \<tau> \<omega> (I \<inter> assertify_bexp (Bnot b))"
+      proof (cases n)
+        case (Suc m)
+        show "safe n C' s \<tau> \<omega> (I \<inter> assertify_bexp (Bnot b))"
+          unfolding Suc
+        proof (rule safeI)
+          show "no_aborts C' s \<omega>"
+            using asm1(1) by blast
+          fix \<omega>0' \<omega>f C'' \<sigma>'
+          assume asm2: "sep_algebra_class.stable \<omega>f" "Some \<omega>0' = \<omega> \<oplus> \<omega>f" "binary_mask \<omega>0'"
+          assume "\<langle>C', concretize s \<omega>0'\<rangle> \<rightarrow> \<langle>C'', \<sigma>'\<rangle>"
+          then show "\<exists>\<omega>1 \<omega>1'. Some \<omega>1' = \<omega>1 \<oplus> \<omega>f \<and> sep_algebra_class.stable \<omega>1 \<and> binary_mask \<omega>1' \<and> snd \<sigma>' = get_vh \<omega>1' \<and> safe m C'' (fst \<sigma>') \<tau> \<omega>1 (I \<inter> assertify_bexp (Bnot b))"
+            unfolding asm1(1)
+          proof (rule red_if_cases)
+            show "C'' = Cskip \<Longrightarrow> \<sigma>' = concretize s \<omega>0' \<Longrightarrow> \<not> bdenot b (fst (concretize s \<omega>0')) \<Longrightarrow>
+    \<exists>\<omega>1 \<omega>1'. Some \<omega>1' = \<omega>1 \<oplus> \<omega>f \<and> sep_algebra_class.stable \<omega>1 \<and> binary_mask \<omega>1' \<and> snd \<sigma>' = get_vh \<omega>1' \<and> safe m C'' (fst \<sigma>') \<tau> \<omega>1 (I \<inter> assertify_bexp (Bnot b))"
+              by (metis IntI SucOuter(3) SucOuter(4) asm2(2) asm2(3) bdenot.simps(3) fst_conv in_assertify_bexp_alt safe_skip snd_conv)
+            assume asm3: "C'' = Cseq C (Cwhile b C)" "\<sigma>' = concretize s \<omega>0'" "bdenot b (fst (concretize s \<omega>0'))"
+            have "safe m C'' s \<tau> \<omega> (I \<inter> assertify_bexp (Bnot b))"
+              unfolding asm3(1)
+            proof (rule safe_seq)
+              show "safe m C s \<tau> \<omega> I"
+                by (metis CSL_def IntI SucOuter(3) SucOuter(4) asm3(3) assms(1) fst_conv in_assertify_bexp_alt)
+              show "\<And>ma \<omega>' s'. ma \<le> m \<and> (Ag s', \<tau>, \<omega>') \<in> I \<and> sep_algebra_class.stable \<omega>' \<Longrightarrow> safe ma (Cwhile b C) s' \<tau> \<omega>' (I \<inter> assertify_bexp (Bnot b))"
+                using Suc Suc.hyps[OF assms(1)] le_SucI safety_mono by fast
+            qed (simp add: \<open>sep_algebra_class.stable \<omega>\<close>)
+            then show "\<exists>\<omega>1 \<omega>1'. Some \<omega>1' = \<omega>1 \<oplus> \<omega>f \<and> sep_algebra_class.stable \<omega>1 \<and> binary_mask \<omega>1' \<and> snd \<sigma>' = get_vh \<omega>1' \<and> safe m C'' (fst \<sigma>') \<tau> \<omega>1 (I \<inter> assertify_bexp (Bnot b))"
+              using SucOuter(4) asm2(2) asm2(3) asm3(2) by auto
+          qed
+        qed (simp_all add: asm1(1))
+      qed (simp)
+      then show "\<exists>\<omega>1 \<omega>1'. Some \<omega>1' = \<omega>1 \<oplus> \<omega>f \<and> sep_algebra_class.stable \<omega>1 \<and> binary_mask \<omega>1' \<and> snd \<sigma>' = get_vh \<omega>1' \<and> safe n C' (fst \<sigma>') \<tau> \<omega>1 (I \<inter> assertify_bexp (Bnot b))"
+        using asm0 Suc.prems(3) asm1(2) by auto
+    qed
+  qed (simp_all)
+qed (simp)
+
+
+proposition rule_while:
+  assumes "CSL (I \<inter> (assertify_bexp b)) C I"
+      and "self_framing I"
+    shows "CSL I (Cwhile b C) (I \<inter> (assertify_bexp (Bnot b)))"
+proof (rule CSL_I)
+  fix n s \<tau> \<omega>
+  assume "(Ag s, \<tau>, \<omega>) \<in> I" "sep_algebra_class.stable \<omega>"
+  then show "safe (Suc n) (Cwhile b C) s \<tau> \<omega> (I \<inter> assertify_bexp (Bnot b))"
+    using assms(1) safe_while by blast
+qed
+
+
+
+
+subsection \<open>Rule FieldAssign\<close>
+
+abbreviation update_heap_val where
+  "update_heap_val \<omega> l v \<equiv> set_state \<omega> (set_value (get_state \<omega>) l v)"
+
+lemma write_helper:
+  assumes "Some \<omega>' = \<omega> \<oplus> \<omega>f"
+      and "sep_algebra_class.stable \<omega>f"
+      and "get_vm \<omega> l = 1"
+    shows "Some (set_value \<omega>' l v) = set_value \<omega> l v \<oplus> \<omega>f"
+proof -
+  have "get_vm \<omega>' l = get_vm \<omega> l + get_vm \<omega>f l"
+    using EquiViper.add_masks_def assms(1) get_vm_additive by blast
+  moreover have "get_vm \<omega>' l \<le> 1" sorry
+  ultimately have "get_vm \<omega>f l = 0"
+    by (metis PosReal.padd_cancellative add.commute add.right_neutral assms(3) nle_le pos_perm_class.sum_larger)
+  moreover have "get_vh \<omega>f l = None"
+    using assms(2) calculation pperm_pgt_pnone stable_virtual_state_def by blast
+  show ?thesis
+  proof (rule compatible_virtual_state_implies_pre_virtual_state_rev)
+    show "Some (Rep_virtual_state (set_value \<omega>' l v)) = Rep_virtual_state (set_value \<omega> l v) \<oplus> Rep_virtual_state \<omega>f"
+    proof (rule plus_prodI)
+      show "Some (fst (Rep_virtual_state (set_value \<omega>' l v))) = fst (Rep_virtual_state (set_value \<omega> l v)) \<oplus> fst (Rep_virtual_state \<omega>f)"
+        by (metis assms(1) get_vm_additive get_vm_def set_value_charact(1))
+      show "Some (snd (Rep_virtual_state (set_value \<omega>' l v))) = snd (Rep_virtual_state (set_value \<omega> l v)) \<oplus> snd (Rep_virtual_state \<omega>f)"
+      proof (rule plus_funI)
+        fix la show "Some (snd (Rep_virtual_state (set_value \<omega>' l v)) la) = snd (Rep_virtual_state (set_value \<omega> l v)) la \<oplus> snd (Rep_virtual_state \<omega>f) la"
+        proof (cases "l = la")
+          case True
+          then have "snd (Rep_virtual_state (set_value \<omega>' l v)) la = Some v"
+            by (metis fun_upd_apply get_vh_def set_value_charact(2))
+          moreover have "snd (Rep_virtual_state (set_value \<omega> l v)) la = Some v"
+            by (metis True fun_upd_apply get_vh_def set_value_charact(2))
+          ultimately show ?thesis
+            by (metis True \<open>get_vh \<omega>f l = None\<close> get_vh_def plus_option.simps(2))
+        next
+          case False
+          then show ?thesis
+            by (metis assms(1) fun_upd_apply get_vh_def plus_funE set_value_charact(2) vstate_add_iff)
+        qed
+      qed
+    qed
+  qed
+qed
+
+
+definition full_ownership :: "var \<Rightarrow> int equi_state set"
+  where
+  "full_ownership r = { \<omega> |\<omega> l. get_store \<omega> r = Some (VRef (Address l)) \<and> get_m \<omega> (l, field_val) = 1}"
+
+definition full_ownership_with_val where
+  "full_ownership_with_val r e = { \<omega> |\<omega> l. get_store \<omega> r = Some (VRef (Address l)) \<and> get_m \<omega> (l, field_val) = 1
+  \<and> get_h \<omega> (l, field_val) = Some (VInt (edenot e (get_store \<omega>)))  }"
+
+lemma in_full_ownership_with_val:
+  assumes "get_store \<omega> r = Some (VRef (Address l))"
+      and "get_m \<omega> (l, field_val) = 1"
+      and "get_h \<omega> (l, field_val) = Some (VInt (edenot e (get_store \<omega>)))"
+    shows "\<omega> \<in> full_ownership_with_val r e"
+  using assms full_ownership_with_val_def by blast
+
+lemma get_simps_unfolded[simp]:
+  "get_store (Ag s, \<tau>, \<omega>) = s"
+  "get_state (Ag s, \<tau>, \<omega>) = \<omega>"
+  "get_h (Ag s, \<tau>, \<omega>) = get_vh \<omega>"
+  "get_m (Ag s, \<tau>, \<omega>) = get_vm \<omega>"
+     apply (simp add: get_store_def)
+      apply (simp add: get_state_def)
+    apply (simp add: get_state_def)
+  by (simp add: get_state_def)
+
+
+lemma in_full_ownership_with_val_alt:
+  assumes "s r = Some (VRef (Address l))"
+      and "get_vm \<omega> (l, field_val) = 1"
+      and "get_vh \<omega> (l, field_val) = Some (VInt (edenot e s))"
+    shows "(Ag s, \<tau>, \<omega>) \<in> full_ownership_with_val r e"
+  unfolding full_ownership_with_val_def
+  using assms by auto
+
+
+lemma in_read_dom_write_dom:
+  assumes "get_vm \<omega> (l, field_val) = 1"
+  shows "l \<in> read_dom \<omega>"
+    and "l \<in> write_dom \<omega>"
+  apply (metis CollectI assms not_gr_0 read_dom_def zero_neq_one)
+  by (simp add: assms write_dom_def)
+
+lemma stable_before_then_update_stable:
+  assumes "sep_algebra_class.stable \<omega>"
+      and "get_vh \<omega> l \<noteq> None"
+  shows "sep_algebra_class.stable (set_value \<omega> l v)"
+  by (metis assms(1) assms(2) fun_upd_apply set_value_charact(1) set_value_charact(2) stable_virtual_state_def)
+
+
+proposition rule_write:
+  "CSL (full_ownership r) (Cwrite r e) (full_ownership_with_val r e)"
+proof (rule CSL_I)
+  fix n s \<tau> \<omega> assume "(Ag s, \<tau>, \<omega>) \<in> full_ownership r" "sep_algebra_class.stable \<omega>"
+  then obtain l where asm0: "s r = Some (VRef (Address l)) \<and> get_vm \<omega> (l, field_val) = 1"
+    using full_ownership_def by fastforce
+  show "safe n (Cwrite r e) s \<tau> \<omega> (full_ownership_with_val r e)"
+  proof (cases n)
+    case (Suc m)
+    moreover have "safe (Suc m) (Cwrite r e) s \<tau> \<omega> (full_ownership_with_val r e)"
+    proof (rule safeI_alt)
+      have "accesses (Cwrite r e) s = {l}" using get_address_simp asm0 by auto
+      then show "accesses (Cwrite r e) s \<subseteq> read_dom \<omega>" using asm0
+        by (simp add: in_read_dom_write_dom(1))
+      show "writes (Cwrite r e) s \<subseteq> write_dom \<omega>"
+        by (simp add: asm0 in_read_dom_write_dom(2))
+      fix \<omega>0' \<omega>f
+      assume asm1: "Some \<omega>0' = \<omega> \<oplus> \<omega>f" "binary_mask \<omega>0'" "sep_algebra_class.stable \<omega>f"
+      then have "s r = Some (VRef (Address l)) \<and> get_vm \<omega>0' (l, field_val) = 1"
+        by (metis EquiViper.add_masks_def asm0 binary_mask_def get_vm_additive padd_pos)
+      then have "get_vh \<omega>0' (l, field_val) \<noteq> None"
+        by (simp add: pperm_pnone_pgt vstate_wf_imp)
+
+      show "aborts (Cwrite r e) (concretize s \<omega>0') \<Longrightarrow> False"
+      proof -
+        assume "aborts (Cwrite r e) (concretize s \<omega>0')"
+        then show False
+          using \<open>get_vh \<omega>0' (l, field_val) \<noteq> None\<close> asm0 by auto
+      qed
+      fix C' \<sigma>'
+      assume asm2: "sep_algebra_class.stable \<omega>f" "\<langle>Cwrite r e, concretize s \<omega>0'\<rangle> \<rightarrow> \<langle>C', \<sigma>'\<rangle>"
+      let ?v = "VInt (edenot e s)"
+
+      have "Some (set_value \<omega>0' (l, field_val) ?v) = set_value \<omega> (l, field_val) ?v \<oplus> \<omega>f"
+        using asm0 asm1 asm2 write_helper by blast
+      moreover have "\<sigma>' = concretize s (set_value \<omega>0' (l, field_val) ?v) \<and> C' = Cskip"
+        using red_write_cases[OF asm2(2)]
+        using \<open>s r = Some (VRef (Address l)) \<and> get_vm \<omega>0' (l, field_val) = PosReal.pwrite\<close> old.prod.inject option.inject ref.inject set_value_charact(2) val.inject(4) by fastforce
+      moreover have "safe m Cskip s \<tau> (set_value \<omega> (l, field_val) ?v) (full_ownership_with_val r e)"
+      proof (rule safe_skip)
+        show "(Ag s, \<tau>, set_value \<omega> (l, field_val) (VInt (edenot e s))) \<in> full_ownership_with_val r e"
+          by (simp add: asm0 asm1 full_add_charact(1) full_ownership_with_val_def)
+      qed
+      ultimately show "\<exists>\<omega>1 \<omega>1'. Some \<omega>1' = \<omega>1 \<oplus> \<omega>f \<and> sep_algebra_class.stable \<omega>1 \<and> binary_mask \<omega>1' \<and> snd \<sigma>' = get_vh \<omega>1' \<and> safe m C' (fst \<sigma>') \<tau> \<omega>1 (full_ownership_with_val r e)"
+        by (metis \<open>sep_algebra_class.stable \<omega>\<close> asm0 asm1(2) binary_mask_def fst_conv not_gr_0 one_neq_zero set_value_charact(1) snd_conv stable_before_then_update_stable vstate_wf_imp)
+    qed (simp)
+    ultimately show ?thesis by blast
+  qed (simp)
+qed
+
+
+subsection \<open>Rule assignment\<close>
+
+(*
+| RuleLocalAssign: "\<lbrakk> self_framing_and_typed \<Delta> A; framed_by_exp A e \<rbrakk> \<Longrightarrow> \<Delta> \<turnstile> [A] LocalAssign x e [post_substitute_var_assert x e A]"
+*)
+(*
+| red_Assign[intro]:"\<lbrakk> \<sigma> = (s,h); \<sigma>' = (s(x \<mapsto> VInt (edenot e s)), h) \<rbrakk> \<Longrightarrow> \<langle>Cassign x e, \<sigma>\<rangle> \<rightarrow> \<langle>Cskip, \<sigma>'\<rangle>"
+*)
+
+definition sub_pre where
+  "sub_pre x e P = { (Ag s, \<tau>, \<omega>) |s \<tau> \<omega>. (Ag (s(x \<mapsto> VInt (edenot e s))), \<tau>, \<omega>) \<in> P }"
+
+proposition rule_assign:
+  "CSL (sub_pre x e P) (Cassign x e) P"
+proof (rule CSL_I)
+  fix n s \<tau> \<omega>
+  assume asm0: "(Ag s, \<tau>, \<omega>) \<in> sub_pre x e P" "sep_algebra_class.stable \<omega>"
+  then have r: "(Ag (s(x \<mapsto> VInt (edenot e s))), \<tau>, \<omega>) \<in> P"
+    by (simp add: sub_pre_def)
+  show "safe (Suc n) (Cassign x e) s \<tau> \<omega> P"
+  proof (rule safeI)
+    fix \<omega>0' \<omega>f C' \<sigma>'
+    assume asm1: "sep_algebra_class.stable \<omega>f" "Some \<omega>0' = \<omega> \<oplus> \<omega>f" "binary_mask \<omega>0'"
+    assume "\<langle>Cassign x e, concretize s \<omega>0'\<rangle> \<rightarrow> \<langle>C', \<sigma>'\<rangle>"
+    then show "\<exists>\<omega>1 \<omega>1'. Some \<omega>1' = \<omega>1 \<oplus> \<omega>f \<and> sep_algebra_class.stable \<omega>1 \<and> binary_mask \<omega>1' \<and> snd \<sigma>' = get_vh \<omega>1' \<and> safe n C' (fst \<sigma>') \<tau> \<omega>1 P"
+      by (metis asm0(2) asm1(2) asm1(3) fst_eqD r red_assign_cases safe_skip snd_eqD)
+  qed (auto simp add: no_aborts_def)
+qed
+
+
+
+subsection \<open>Rule Alloc\<close>
+
+definition set_perm_and_value :: "'a virtual_state \<Rightarrow> (address \<times> field_ident) \<Rightarrow> preal \<Rightarrow> 'a val option \<Rightarrow> 'a virtual_state" where
+  "set_perm_and_value \<phi> hl p v = Abs_virtual_state ((get_vm \<phi>)(hl := p), (get_vh \<phi>)(hl := v))"
+
+(* Not true, needs pre... *)
+lemma wf_set_perm:
+  assumes "p > 0 \<Longrightarrow> v \<noteq> None"
+  shows "wf_pre_virtual_state ((get_vm \<phi>)(hl := p), (get_vh \<phi>)(hl := v))"
+  using assms gr_0_is_ppos vstate_wf_imp by fastforce
+
+lemma update_perm_simps[simp]:
+  assumes "p > 0 \<Longrightarrow> v \<noteq> None"
+    shows "get_vh (set_perm_and_value \<phi> hl p v) = (get_vh \<phi>)(hl := v)"
+      and "get_vm (set_perm_and_value \<phi> hl p v) = (get_vm \<phi>)(hl := p)"
+  unfolding set_perm_and_value_def
+  apply (metis Abs_virtual_state_inverse assms get_vh_def mem_Collect_eq snd_conv wf_set_perm)
+  by (metis Abs_virtual_state_inverse assms fst_conv get_vm_def mem_Collect_eq wf_set_perm)
+
+lemma stable_set_perm_and_value:
+  assumes "p > 0 \<longleftrightarrow> v \<noteq> None"
+      and "stable \<omega>"
+    shows "stable (set_perm_and_value \<omega> hl p v)"
+proof (rule stable_virtual_stateI)
+  show "\<And>hla. get_vh (set_perm_and_value \<omega> hl p v) hla \<noteq> None \<Longrightarrow> PosReal.pnone < get_vm (set_perm_and_value \<omega> hl p v) hla"
+    by (metis assms(1) assms(2) fun_upd_apply stable_virtual_state_def update_perm_simps(1) update_perm_simps(2))
+qed
+
+lemma plus_virtual_stateI:
+  assumes "Some (get_vh \<phi>) = get_vh a \<oplus> get_vh b"
+      and "Some (get_vm \<phi>) = get_vm a \<oplus> get_vm b"
+    shows "Some \<phi> = a \<oplus> b"
+  using assms(1) assms(2) vstate_add_iff by blast
+
+
+
+lemma alloc_helper:
+  assumes "Some \<omega>' = \<omega> \<oplus> \<omega>f"
+      and "get_vh \<omega>f l = None"
+      and "p > 0 \<Longrightarrow> v \<noteq> None"
+    shows "Some (set_perm_and_value \<omega>' l p v) = set_perm_and_value \<omega> l p v \<oplus> \<omega>f"
+proof (rule plus_virtual_stateI)
+  show "Some (get_vh (set_perm_and_value \<omega>' l p v)) = get_vh (set_perm_and_value \<omega> l p v) \<oplus> get_vh \<omega>f"
+    by (smt (verit, ccfv_threshold) assms commutative fun_upd_apply plus_funE plus_funI plus_option.simps(1) update_perm_simps(1) vstate_add_iff)
+  show "Some (get_vm (set_perm_and_value \<omega>' l p v)) = get_vm (set_perm_and_value \<omega> l p v) \<oplus> get_vm \<omega>f"
+    apply (rule plus_funI)
+    by (smt (verit, ccfv_threshold) SepAlgebra.plus_preal_def add.right_neutral assms fun_upd_apply get_vm_additive not_gr_0 plus_funE update_perm_simps(2) vstate_wf_imp)
+qed
+
+
+proposition rule_alloc:
+  assumes "r \<notin> fvE e"
+  shows "CSL UNIV (Calloc r e) (full_ownership_with_val r e)"
+proof (rule CSL_I)
+  fix n :: nat
+  fix s :: stack
+  fix \<tau> :: "int ag_trace"
+  fix \<omega> :: "int virtual_state"
+  assume "sep_algebra_class.stable \<omega>"
+
+
+  show "safe (Suc n) (Calloc r e) s \<tau> \<omega> (full_ownership_with_val r e)"
+  proof (rule safeI)
+    fix \<omega>0' \<omega>f C' \<sigma>'
+    assume asm0: "sep_algebra_class.stable \<omega>f" "Some \<omega>0' = \<omega> \<oplus> \<omega>f" "binary_mask \<omega>0'"
+    assume "\<langle>Calloc r e, concretize s \<omega>0'\<rangle> \<rightarrow> \<langle>C', \<sigma>'\<rangle>"
+    then show "\<exists>\<omega>1 \<omega>1'. Some \<omega>1' = \<omega>1 \<oplus> \<omega>f \<and> sep_algebra_class.stable \<omega>1 \<and> binary_mask \<omega>1' \<and> snd \<sigma>' = get_vh \<omega>1' \<and> safe n C' (fst \<sigma>') \<tau> \<omega>1 (full_ownership_with_val r e)"
+    proof (rule red_alloc_cases)
+      fix sa h l
+      assume asm1: "concretize s \<omega>0' = (sa, h)" "C' = Cskip" "(l, field_val) \<notin> dom h"
+        "\<sigma>' = (sa(r \<mapsto> VRef (Address l)), h((l, field_val) \<mapsto> VInt (edenot e sa)))"
+      then have r: "Some (set_perm_and_value \<omega>0' (l, field_val) 1 (Some (VInt (edenot e s))))
+  = set_perm_and_value \<omega> (l, field_val) 1 (Some (VInt (edenot e s))) \<oplus> \<omega>f"
+        using alloc_helper
+        by (smt (verit, ccfv_SIG) EquiViper.add_masks_def Pair_inject asm0(1) asm0(2) commutative dom_eqD option.discI padd_pos pperm_pnone_pgt stable_virtual_state_def vstate_add_iff vstate_wf_imp)
+      let ?\<omega>1 = "set_perm_and_value \<omega> (l, field_val) 1 (Some (VInt (edenot e s)))"
+      let ?\<omega>1' = "set_perm_and_value \<omega>0' (l, field_val) 1 (Some (VInt (edenot e s)))"
+
+      have "sep_algebra_class.stable ?\<omega>1"
+        by (simp add: \<open>sep_algebra_class.stable \<omega>\<close> pperm_pnone_pgt stable_set_perm_and_value)
+      moreover have "binary_mask ?\<omega>1'"
+      proof (rule binary_maskI)
+        fix la show "get_vm (set_perm_and_value \<omega>0' (l, field_val) PosReal.pwrite (Some (VInt (edenot e s)))) la = PosReal.pnone \<or>
+          get_vm (set_perm_and_value \<omega>0' (l, field_val) PosReal.pwrite (Some (VInt (edenot e s)))) la = PosReal.pwrite"
+          by (metis asm0(3) binary_mask_def fun_upd_apply option.discI update_perm_simps(2))
+      qed
+      moreover have "\<sigma>' = concretize (fst \<sigma>') ?\<omega>1'"
+        using asm1(1) asm1(4) by auto
+      moreover have "(Ag (fst \<sigma>'), \<tau>, ?\<omega>1) \<in> full_ownership_with_val r e"
+      proof (rule in_full_ownership_with_val_alt[of "(fst \<sigma>')" r l])
+        show "fst \<sigma>' r = Some (VRef (Address l))"
+          by (simp add: asm1(4))
+        show "get_vm (set_perm_and_value \<omega> (l, field_val) PosReal.pwrite (Some (VInt (edenot e s)))) (l, field_val) = PosReal.pwrite"
+          by auto
+        have "edenot e (fst \<sigma>') = edenot e s"
+          using asm1(1) asm1(4) assms by auto
+        then show "get_vh (set_perm_and_value \<omega> (l, field_val) PosReal.pwrite (Some (VInt (edenot e s)))) (l, field_val)
+          = Some (VInt (edenot e (fst \<sigma>')))"
+          by simp
+      qed
+      ultimately show "\<exists>\<omega>1 \<omega>1'. Some \<omega>1' = \<omega>1 \<oplus> \<omega>f \<and> sep_algebra_class.stable \<omega>1 \<and> binary_mask \<omega>1' \<and> snd \<sigma>' = get_vh \<omega>1' \<and> safe n C' (fst \<sigma>') \<tau> \<omega>1 (full_ownership_with_val r e)"
+        using r asm1(2)
+        by (metis safe_skip snd_conv)
+    qed
+  qed (auto)
+qed
+
+
+
+subsection \<open>Rule free\<close>
+
+definition erase_perm_and_value :: "'a virtual_state \<Rightarrow> (address \<times> field_ident) \<Rightarrow> 'a virtual_state" where
+  "erase_perm_and_value \<phi> hl = Abs_virtual_state ((get_vm \<phi>)(hl := 0), (get_vh \<phi>)(hl := None))"
+
+lemma erase_perm_and_value_simps[simp]:
+  "get_vm (erase_perm_and_value \<phi> hl) = (get_vm \<phi>)(hl := 0)"
+  "get_vh (erase_perm_and_value \<phi> hl) = (get_vh \<phi>)(hl := None)"
+proof -
+  show "get_vm (erase_perm_and_value \<phi> hl) = (get_vm \<phi>)(hl := PosReal.pnone)"
+    by (metis erase_perm_and_value_def pperm_pgt_pnone set_perm_and_value_def update_perm_simps(2))
+  show "get_vh (erase_perm_and_value \<phi> hl) = (get_vh \<phi>)(hl := None)"
+    by (metis erase_perm_and_value_def pperm_pgt_pnone set_perm_and_value_def update_perm_simps(1))
+qed
+
+
+lemma free_helper:
+  assumes "Some \<omega>' = \<omega> \<oplus> \<omega>f"
+      and "sep_algebra_class.stable \<omega>f"
+      and "get_vm \<omega> hl = 1"
+    shows "Some (erase_perm_and_value \<omega>' hl) = erase_perm_and_value \<omega> hl \<oplus> \<omega>f"
+proof -
+  have asm: "get_vm \<omega>' hl = 1"
+    sorry
+  then have "get_vm \<omega>f hl = 0"
+    by (smt (verit, ccfv_threshold) EquiViper.add_masks_def PosReal.ppos.rep_eq assms(1) assms(3) get_vm_additive gr_0_is_ppos not_gr_0 plus_preal.rep_eq)
+  then have "get_vh \<omega>f hl = None"
+    using assms(2) pperm_pgt_pnone stable_virtual_state_def by blast
+  show ?thesis
+  proof (rule plus_virtual_stateI)
+    show "Some (get_vh (erase_perm_and_value \<omega>' hl)) = get_vh (erase_perm_and_value \<omega> hl) \<oplus> get_vh \<omega>f"
+      by (metis \<open>get_vh \<omega>f hl = None\<close> alloc_helper assms(1) erase_perm_and_value_def pperm_pgt_pnone set_perm_and_value_def vstate_add_iff)
+    show "Some (get_vm (erase_perm_and_value \<omega>' hl)) = get_vm (erase_perm_and_value \<omega> hl) \<oplus> get_vm \<omega>f"
+      by (metis \<open>get_vh \<omega>f hl = None\<close> alloc_helper assms(1) erase_perm_and_value_def pperm_pgt_pnone set_perm_and_value_def vstate_add_iff)
+  qed
+qed
+
+lemma stable_erase_perm_value:
+  assumes "sep_algebra_class.stable \<omega>"
+  shows "sep_algebra_class.stable (erase_perm_and_value \<omega> hl)"
+  by (metis assms erase_perm_and_value_def order_less_irrefl set_perm_and_value_def stable_set_perm_and_value)
+
+lemma binary_mask_erase_perm_value:
+  assumes "binary_mask \<omega>"
+  shows "binary_mask (erase_perm_and_value \<omega> hl)"
+  by (metis assms binary_mask_def erase_perm_and_value_simps(1) fun_upd_def)
+
+
+proposition rule_free:
+  "CSL (full_ownership r) (Cfree r) UNIV"
+proof (rule CSL_I)
+  fix n s \<tau> \<omega>
+  assume asm0: "(Ag s, \<tau>, \<omega>) \<in> full_ownership r" "sep_algebra_class.stable \<omega>"
+  then obtain l where r: "s r = Some (VRef (Address l)) \<and> get_vm \<omega> (l, field_val) = 1"
+    using full_ownership_def by fastforce
+  show "safe (Suc n) (Cfree r) s \<tau> \<omega> UNIV"
+  proof (rule safeI_alt)
+    show "accesses (Cfree r) s \<subseteq> read_dom \<omega>"
+      by (simp add: in_read_dom_write_dom(1) r)
+    show "writes (Cfree r) s \<subseteq> write_dom \<omega>"
+      by (simp add: in_read_dom_write_dom(2) r)
+    fix \<omega>0' \<omega>f
+    assume asm1: "sep_algebra_class.stable \<omega>f" "Some \<omega>0' = \<omega> \<oplus> \<omega>f" "binary_mask \<omega>0'"
+    show "aborts (Cfree r) (concretize s \<omega>0') \<Longrightarrow> False"
+    proof -
+      assume "aborts (Cfree r) (concretize s \<omega>0')"
+      then show False
+      proof (rule aborts_free_elim)
+        show "fst (concretize s \<omega>0') r = Some (VRef Null) \<Longrightarrow> False"
+          by (simp add: r)
+        fix hl assume "fst (concretize s \<omega>0') r = Some (VRef (Address hl))"
+        then have "hl = l"
+          by (simp add: r)
+        moreover have "get_vm \<omega>0' (l, field_val) \<ge> 1"
+          by (simp add: EquiViper.add_masks_def asm1(2) get_vm_additive pos_perm_class.sum_larger r)
+        moreover assume "(hl, field_val) \<notin> dom (snd (concretize s \<omega>0'))"
+        ultimately show False
+          by (metis domIff linorder_not_less pperm_pnone_pgt sndI vstate_wf_imp zero_neq_one)
+      qed
+    qed
+    fix C' \<sigma>'
+    assume "\<langle>Cfree r, concretize s \<omega>0'\<rangle> \<rightarrow> \<langle>C', \<sigma>'\<rangle>"
+    then show "\<exists>\<omega>1 \<omega>1'. Some \<omega>1' = \<omega>1 \<oplus> \<omega>f \<and> sep_algebra_class.stable \<omega>1 \<and> binary_mask \<omega>1' \<and> snd \<sigma>' = get_vh \<omega>1' \<and> safe n C' (fst \<sigma>') \<tau> \<omega>1 UNIV"
+    proof (rule red_free_cases)
+      fix sa h l'
+      assume asm2: "concretize s \<omega>0' = (sa, h)" "C' = Cskip" "\<sigma>' = (sa, h((l', field_val) := None))"
+        "sa r = Some (VRef (Address l'))"
+      let ?\<omega>1 = "erase_perm_and_value \<omega> (l', field_val)"
+      let ?\<omega>1' = "erase_perm_and_value \<omega>0' (l', field_val)"
+      have "snd \<sigma>' = get_vh ?\<omega>1' \<and> safe n C' (fst \<sigma>') \<tau> ?\<omega>1 UNIV"
+        using asm2(1) asm2(2) asm2(3) by auto
+      moreover have "Some ?\<omega>1' = ?\<omega>1 \<oplus> \<omega>f \<and> sep_algebra_class.stable ?\<omega>1"
+        using asm0(2) asm1(1) asm1(2) asm2(1) asm2(4) free_helper r stable_erase_perm_value by fastforce
+      moreover have "binary_mask ?\<omega>1'"
+        by (simp add: asm1(3) binary_mask_erase_perm_value)        
+      ultimately show
+        "\<exists>\<omega>1 \<omega>1'. Some \<omega>1' = \<omega>1 \<oplus> \<omega>f \<and> sep_algebra_class.stable \<omega>1 \<and> binary_mask \<omega>1' \<and> snd \<sigma>' = get_vh \<omega>1' \<and> safe n C' (fst \<sigma>') \<tau> \<omega>1 UNIV"
+        by blast
+    qed
+  qed (simp_all)
+qed
+
+
+subsection \<open>Read\<close>
+
+lemma read_helper:
+  assumes "Some \<omega>' = \<omega> \<oplus> \<omega>f"
+      and "get_vh \<omega> l = Some v"
+    shows "get_vh \<omega>' l = Some v"
+  by (metis assms(1) assms(2) commutative greater_equiv read_field.elims read_field_mono)
+
+
+
+definition read_result where
+  "read_result x r = { \<omega> |\<omega> l. get_store \<omega> r = Some (VRef (Address l)) \<and> get_store \<omega> x = get_h \<omega> (l, field_val) }"
+
+proposition rule_read:
+  assumes "x \<notin> fvA A"
+      and "\<And>\<omega>. \<omega> \<in> A \<Longrightarrow> (\<exists>l v. get_store \<omega> r = Some (VRef (Address l)) \<and> get_m \<omega> (l, field_val) > 0 \<and> get_h \<omega> (l, field_val) = Some (VInt v))"
+    shows "CSL A (Cread x r) (A \<inter> read_result x r)"
+proof (rule CSL_I)
+  fix n s \<tau> \<omega>
+  assume asm0: "(Ag s, \<tau>, \<omega>) \<in> A" "sep_algebra_class.stable \<omega>"
+  then obtain l v where lv_def: "s r = Some (VRef (Address l))" "get_vm \<omega> (l, field_val) > 0" "get_vh \<omega> (l, field_val) = Some (VInt v)"
+    using assms(2) by force
+  show "safe (Suc n) (Cread x r) s \<tau> \<omega> (A \<inter> read_result x r)"
+  proof (rule safeI_alt)
+    show "accesses (Cread x r) s \<subseteq> read_dom \<omega>"
+      by (simp add: lv_def(1) lv_def(2) read_dom_def)
+    fix \<omega>0' \<omega>f
+    assume asm1: "sep_algebra_class.stable \<omega>f" "Some \<omega>0' = \<omega> \<oplus> \<omega>f" "binary_mask \<omega>0'"
+    then have "get_vh \<omega>0' (l, field_val) = Some (VInt v)"
+      using lv_def(3) read_helper by blast
+    then show "aborts (Cread x r) (concretize s \<omega>0') \<Longrightarrow> False"
+      using lv_def(1) by auto
+    have "(Ag (s(x := Some (VInt v))), \<tau>, \<omega>) \<in> A"
+      by (meson agrees_search(4) asm0(1) assms(1) fvA_agrees)
+
+    fix C' \<sigma>'
+    assume "\<langle>Cread x r, concretize s \<omega>0'\<rangle> \<rightarrow> \<langle>C', \<sigma>'\<rangle>"
+    then show "\<exists>\<omega>1 \<omega>1'. Some \<omega>1' = \<omega>1 \<oplus> \<omega>f \<and> sep_algebra_class.stable \<omega>1 \<and> binary_mask \<omega>1' \<and> snd \<sigma>' = get_vh \<omega>1' \<and> safe n C' (fst \<sigma>') \<tau> \<omega>1 (A \<inter> read_result x r)"
+    proof (rule red_read_cases)
+      fix sa h l' v'
+      assume asm2: "concretize s \<omega>0' = (sa, h)" "C' = Cskip" "\<sigma>' = (sa(x \<mapsto> VInt v'), h)" "sa r = Some (VRef (Address l'))"
+      "h (l', field_val) = Some (VInt v')"
+      then have "l = l' \<and> v = v'"
+        using \<open>get_vh \<omega>0' (l, field_val) = Some (VInt v)\<close> lv_def(1) by auto
+      moreover have "(Ag (s(x := Some (VInt v))), \<tau>, \<omega>) \<in> read_result x r"
+        unfolding read_result_def
+        using \<open>(Ag (s(x \<mapsto> VInt v)), \<tau>, \<omega>) \<in> A\<close> assms(2) get_simps_unfolded(1) lv_def(1) lv_def(3) by fastforce
+      ultimately show "\<exists>\<omega>1 \<omega>1'. Some \<omega>1' = \<omega>1 \<oplus> \<omega>f \<and> sep_algebra_class.stable \<omega>1 \<and> binary_mask \<omega>1' \<and> snd \<sigma>' = get_vh \<omega>1' \<and> safe n C' (fst \<sigma>') \<tau> \<omega>1 (A \<inter> read_result x r)"
+        using \<open>(Ag (s(x \<mapsto> VInt v)), \<tau>, \<omega>) \<in> A\<close> asm0(2) asm1(2) asm1(3) asm2(1) asm2(2) asm2(3) by auto
+    qed
+  qed (simp_all)
+qed
+
 
 
 end
